WIP

qtesla/code/Hacl.Impl.QTesla.Globals.fst
@@ -15,20 +15,33 @@ open Hacl.Impl.QTesla.Lemmas
 
 module UI32 = FStar.UInt32
 module I64 = FStar.Int64
+module I32 = FStar.Int32
 
 #reset-options "--z3rlimit 100 --max_fuel 0 --max_ifuel 0"
 
-// elem_base and uelem_base are defined per parameter set, but because the real definition needs to
-// reference params_q, we actually define the elem and uelem types here.
-let is_elem (#etype:Type0) (e:etype) = 
-  let q = elem_v params_q in
-  let x:int = match etype with
-            | elem -> elem_v e
-            | I64.t -> I64.v e
-            | I32.t -> I32.v e in
-in  -q < x /\ x < q
+//let is_elem (e:elem_base) = let x = elem_v e in let q = elem_v params_q in -q < x /\ x < q
 
-let is_elem e = let x = elem_v e in let q = elem_v params_q in -q < x /\ x < q
+let is_elem_int (e:int) : GTot bool =
+  let q = elem_v params_q in
+  -q < e && e < q
+
+(*assume IntTypeInequality : ~(I32.t == I64.t) /\ ~(I32.t == int) /\ ~(I64.t == int) 
+
+let is_elem (#a:Type) (e:a) =
+  let q = elem_v params_q in
+  (a == I64.t \/ a == I32.t \/ a == int) /\
+  ((a == I32.t) ==> (let x = I32.v e in is_elem_int x)) /\
+  ((a == I64.t) ==> (let x = I64.v e in is_elem_int x)) /\
+  ((a == int) ==> (is_elem_int e))*)
+
+let is_elem (e:elem_base) : GTot bool = let x = elem_v e in is_elem_int x
+let is_elem_i32 (e:I32.t) : GTot bool = let x = I32.v e in is_elem_int x
+let is_elem_i64 (e:I64.t) : GTot bool = let x = I64.v e in is_elem_int x
+
+//let test _ = let e:I32.t = 0l in assert(is_elem e)
+
+//#reset-options "--z3rlimit 100 --max_fuel 0 --max_ifuel 0"
+
 type elem = e:elem_base{is_elem e}
 let is_uelem e = let x = uelem_v e in let q = elem_v params_q in 0 <= x /\ x < q
 type uelem = e:uelem_base{is_uelem e}
@@ -39,7 +52,7 @@ val poly_create:
     unit
   -> StackInline poly
     (requires fun _ -> True)
-    (ensures fun _ _ _ -> True)
+    (ensures fun h0 r h1 -> live h1 r /\ stack_allocated r h0 h1 (Seq.create (v params_n) (to_elem 0)))
 
 let poly_create _ = create params_n (to_elem 0)
 
@@ -47,21 +60,22 @@ val poly_k_create:
     unit
   -> StackInline poly_k
     (requires fun _ -> True)
-    (ensures fun _ _ _ -> True)
+    (ensures fun h0 r h1 -> live h1 r /\ stack_allocated r h0 h1 (Seq.create (v params_n * v params_k) (to_elem 0)))
 
 let poly_k_create _ = create (params_n *. params_k) (to_elem 0)
 
-val get_poly: p: poly_k -> k: size_t{k <. params_k} -> GTot poly
+unfold val get_poly: p: poly_k -> k: size_t{k <. params_k} -> GTot poly
 let get_poly p k = gsub p (k *. params_n) params_n
 
-inline_for_extraction
+unfold inline_for_extraction noextract
 val index_poly: p: poly_k -> k: size_t{k <. params_k} -> Stack poly
     (requires fun h -> live h p)
-    (ensures fun h0 pk h1 -> h0 == h1 /\ pk == get_poly p k)
+    (ensures  fun h0 r h1 -> h0 == h1 /\ live h1 r /\ r == gsub p (size (v k * v params_n)) params_n /\
+                          loc_includes (loc p) (loc r))
 let index_poly p k = sub p (k *. params_n) params_n
 
 val reduce:
-    a: I64.t{FStar.Int.fits (I64.v a * I64.v params_qinv) 64}
+    a: I64.t{FStar.Int.fits (I64.v a * I64.v params_qinv) I64.n}
   -> Tot elem
 
 let reduce a =
@@ -70,15 +84,38 @@ let reduce a =
     lemma_logand32_value_min I64.(a *^ params_qinv);
     let u:I64.t = I64.(u *^ (elem_to_int64 params_q)) in
     let a:I64.t = I64.(a +^ u) in
-    // TODO: need a more specific refinement on a above that lets us prove the result is an elem
     assume(let result = I64.v I64.(a >>^ 32ul) in let q = elem_v params_q in -q < result /\ result < q);
     int64_to_elem I64.(a >>^ 32ul)
 
 val barr_reduce:
-    a: elem
+    a: elem_base
   -> Tot elem
 
 let barr_reduce a =
     let a64:I64.t = elem_to_int64 a in
     let u:elem_base = (int64_to_elem I64.((a64 *^ params_barr_mult) >>^ params_barr_div)) in
+    assume(FStar.Int.fits (elem_v u * elem_v params_q) elem_n);
+    assume(is_elem_int (elem_v a - elem_v u * elem_v params_q));
     a -^ u *^ params_q
+
+(** Modification four buffers -- taken from Lib.Buffer.fsti *)
+let modifies4 (#a0:Type0) (#a1:Type0) (#a2:Type0) (#a3:Type0)
+  (b0:buffer_t MUT a0) (b1:buffer_t MUT a1) (b2:buffer_t MUT a2) (b3:buffer_t MUT a3) (h1 h2: HyperStack.mem) =
+  modifies (loc b0 |+| loc b1 |+| loc b2 |+| loc b3) h1 h2
+
+#reset-options "--z3rlimit 100 --max_fuel 0 --max_ifuel 1"
+
+inline_for_extraction noextract
+val unsafe_declassify:
+    #t:inttype
+  -> us: uint_t t SEC
+  -> Tot (up:uint_t t PUB{uint_v us == uint_v up})
+
+let unsafe_declassify #t us =
+    match t with
+    | U1   -> Lib.RawIntTypes.u8_to_UInt8 (cast U8 SEC us)
+    | U8   -> Lib.RawIntTypes.u8_to_UInt8 us
+    | U16  -> Lib.RawIntTypes.u16_to_UInt16 us
+    | U32  -> Lib.RawIntTypes.u32_to_UInt32 us
+    | U64  -> Lib.RawIntTypes.u64_to_UInt64 us
+    | U128 -> Lib.RawIntTypes.u128_to_UInt128 us
