qtesla/code/Hacl.Impl.QTesla.Heuristic.Poly.fst
@@ -2,6 +2,7 @@ module Hacl.Impl.QTesla.Heuristic.Poly
 
 open FStar.HyperStack
 open FStar.HyperStack.ST
+module ST = FStar.HyperStack.ST
 open FStar.Mul
 
 module I = FStar.Int
@@ -19,16 +20,112 @@ open LowStar.Buffer
 open Lib.IntTypes
 open Lib.Buffer
 open Lib.ByteBuffer
+module LL = Lib.Loops
 
 open C.Loops
+module CL = C.Loops
 
 open Hacl.Impl.QTesla.Params
 open Hacl.Impl.QTesla.Platform
 open Hacl.Impl.QTesla.Constants
 open Hacl.Impl.QTesla.Globals
+open Hacl.Impl.QTesla.Lemmas
 
-#reset-options "--z3rlimit 100 --max_fuel 0 --max_ifuel 0 --admit_smt_queries true"
+#reset-options "--z3rlimit 100 --max_fuel 0 --max_ifuel 0"
 
+inline_for_extraction noextract private
+val ntt_innerfor:
+    numoProblems: size_t{v numoProblems > 0 /\ v numoProblems <= v params_n / 2}
+  -> jFirst: size_t{v jFirst + 2 * v numoProblems <= v params_n}
+  -> a: poly
+  -> wj: elem
+  -> Stack size_t
+    (requires fun h -> live h a)
+    (ensures fun h0 r h1 -> modifies1 a h0 h1 /\ v r = v jFirst + v numoProblems)
+
+let ntt_innerfor numoProblems jFirst a wj =
+    push_frame();
+    let jBuf = create (size 1) jFirst in
+    let liveness h = live h jBuf /\ live h a in
+    let h0 = ST.get() in
+    LL.while
+        (fun h -> liveness h /\ modifies2 a jBuf h0 h /\ v (bget h jBuf 0) <= v jFirst + v numoProblems)
+        (fun h -> v (bget h jBuf 0) < v jFirst + v numoProblems)
+        (fun _ -> jBuf.(size 0) <. jFirst +. numoProblems)
+        (fun _ ->
+            let j = jBuf.(size 0) in
+            let jNumo = j +. numoProblems in
+            let ajNumo:elem = a.(jNumo) in // a[j + NumoProblems]
+            let h1 = ST.get() in
+            lemma_elem_product_fits_int64 wj (bget h1 a (v jNumo));
+            let product = I64.((elem_to_int64 wj) *^ (elem_to_int64 ajNumo)) in
+            assume(FStar.Int.fits (I64.v product * I64.v params_qinv) I64.n);
+            let temp:elem = reduce product in
+            let aj:elem = a.(j) in
+            assume(is_elem_int (elem_v aj - elem_v temp));
+            a.(jNumo) <- aj -^ temp;
+            assume(is_elem_int (elem_v temp + elem_v aj));
+            a.(j) <- temp +^ aj;
+	    jBuf.(size 0) <- j +. size 1;
+            let h2 = ST.get() in
+            let newjVal = v (bget h2 jBuf 0) in
+            assert(newjVal <= v jFirst + v numoProblems)
+        );
+    let h2 = ST.get() in
+    assert(v (bget h2 jBuf 0) = v jFirst + v numoProblems);
+    let res = jBuf.(size 0) in
+    pop_frame();
+    assert(v res = v jFirst + v numoProblems);
+    res
+
+inline_for_extraction noextract private
+val ntt_middlefor:
+    numoProblems: size_t{v numoProblems > 0 /\ v numoProblems <= v params_n / 2}
+  -> jTwiddle: lbuffer size_t (size 1)
+  -> w: poly
+  -> a: poly
+  -> Stack unit
+    (requires fun h -> live h jTwiddle /\ live h w /\ live h a /\
+                    disjoint jTwiddle w /\ disjoint jTwiddle a /\ disjoint w a /\
+                    v (bget h jTwiddle 0) < v params_n - (v params_n / (2 * v numoProblems)))
+    (ensures fun h0 _ h1 -> modifies2 a jTwiddle h0 h1 /\
+                         v (bget h1 jTwiddle 0) = v (bget h0 jTwiddle 0) + (v params_n / (2 * v numoProblems)))
+
+let ntt_middlefor numoProblems jTwiddle w a =
+    push_frame();
+    let jFirst = create (size 1) (size 0) in
+    let h0 = ST.get() in
+    assert(v (bget h0 jTwiddle 0) < v params_n);
+    LL.while
+        (fun h -> live h jTwiddle /\ live h jFirst /\ live h a /\ live h w /\ modifies3 a jTwiddle jFirst h0 h)// /\
+               //(v (bget h jFirst 0) < v params_n ==> v (bget h jTwiddle 0) < v params_n))
+        (fun h -> v (bget h jFirst 0) < v params_n)
+        (fun _ -> jFirst.(size 0) <. params_n)
+        (fun _ ->
+            let h0 = ST.get() in
+            (* Proof note: This loop runs (params_n/(2*numoProblems)) times. Both are always powers of 2 and numoProblems
+             * is always smaller by at least one factor of 2, going all the way down to 1. jTwiddle has been incremented
+             * by (params_n/2*numoProblems) by the time the loop ends.
+             *)
+            let jTwiddleVal = jTwiddle.(size 0) in
+            assume(v jTwiddleVal < v params_n);
+            let wj:elem = w.(jTwiddleVal) in
+            jTwiddle.(size 0) <- jTwiddleVal +. size 1;
+            let h1 = ST.get() in
+            assume(v (bget h1 jFirst 0) + 2 * v numoProblems <= v params_n);
+            // The reference code uses the value for j to increment jFirst, so we follow suit, but j is always
+            // equal to the previous value of jFirst + numoProblems.
+            let j = ntt_innerfor numoProblems jFirst.(size 0) a wj in
+            let h2 = ST.get() in
+            assert(v j = v (bget h2 jFirst 0) + v numoProblems);
+            jFirst.(size 0) <- j +. numoProblems;
+            let h3 = ST.get() in
+            assert(v (bget h3 jFirst 0) = v (bget h2 jFirst 0) + 2 * v numoProblems)
+        );
+    let h3 = ST.get() in
+    assume(v (bget h3 jTwiddle 0) = v (bget h0 jTwiddle 0) + (v params_n / (2 * v numoProblems)));
+    pop_frame()
+        
 val ntt:
     a: poly
   -> w: poly
@@ -40,54 +137,111 @@ let ntt a w =
     push_frame();
     let numoProblems = create (size 1) (params_n >>. (size 1)) in
     let jTwiddle = create (size 1) (size 0) in
-
-    while // Outermost for loop
-        #(fun h -> live h numoProblems /\ live h jTwiddle /\ live h a /\ live h w)
-        #(fun _ h -> live h numoProblems /\ live h jTwiddle /\ live h a /\ live h w)
+    let h0 = ST.get() in
+    LL.while
+        (fun h -> live h numoProblems /\ live h jTwiddle /\ live h a /\ live h w /\ modifies3 numoProblems jTwiddle a h0 h /\
+               v (bget h numoProblems 0) <= (v params_n / 2))
+        (fun h -> v (bget h numoProblems 0) > 0)
         (fun _ -> numoProblems.(size 0) >. (size 0))
         (fun _ ->
-            push_frame();
-            let jBuf = create (size 1) (size 0) in
-            let jFirst = create (size 1) (size 0) in            
-            let cond () : Stack bool
-              (requires fun h -> live h jFirst)
-              (ensures fun h0 _ h1 -> live h1 jFirst)
-            = jFirst.(size 0) <. params_n in
-            while // Middle for loop
-                #(fun h -> live h numoProblems /\ live h jTwiddle /\ live h jBuf /\ live h jFirst /\ live h a /\ live h w)
-                #(fun _ h -> live h numoProblems /\ live h jTwiddle /\ live h jBuf /\ live h jFirst /\ live h a /\ live h w)
-                cond
-                (fun _ ->
-                    let jTwiddleVal = jTwiddle.(size 0) in
-                    let wj_elem = w.(jTwiddleVal) in
-                    let wj:sdigit_t = elem_to_sdigit wj_elem in
-                    jTwiddle.(size 0) <- jTwiddleVal +. (size 1);
-                    // Innermost for loop. Have to use a while because the middle for loop's increment depends on the
-                    // final value of j from each inner for loop, so its scope can't be constrained to the for loop.
-                    jBuf.(size 0) <- jFirst.(size 0);
-                    let jFinish = jFirst.(size 0) +. numoProblems.(size 0) in
-                    while
-                        #(fun h -> live h numoProblems /\ live h jTwiddle /\ live h jFirst /\ live h a /\ live h w /\ live h jBuf)
-                        #(fun _ h -> live h numoProblems /\ live h jTwiddle /\ live h jFirst /\ live h a /\ live h w /\ live h jBuf)
-                        (fun _ -> jBuf.(size 0) <. jFinish)
-                        (fun _ ->
-                            let j = jBuf.(size 0) in
-                            let jNumo = j +. numoProblems.(size 0) in
-                            let ajNumo:elem = a.(jNumo) in // a[j + NumoProblems]
-                            let temp:elem = reduce I64.((sdigit_to_int64 wj) *^ (elem_to_int64 ajNumo)) in
-                            let aj:elem = a.(j) in
-                            a.(jNumo) <- aj -^ temp;
-                            a.(j) <- temp +^ aj;
-			    jBuf.(size 0) <- j +. size 1
-                        );
-                    jFirst.(size 0) <- jBuf.(size 0) +. numoProblems.(size 0)
-                );
-            numoProblems.(size 0) <- numoProblems.(size 0) >>. size 1;
-            pop_frame()
+        (* Proof note: We need to track the value of jTwiddle. This loop will always run for log2(params_n) + 1 iterations.
+         * Each call to ntt_middlefor increments jTwiddle by (params_n/(2*numoProblems)). Need to prove this is always < params_n.
+         *)
+            let h1 = ST.get() in
+            assume(v (bget h1 jTwiddle 0) < v params_n - (v params_n / (2 * v (bget h1 numoProblems 0))));
+            ntt_middlefor numoProblems.(size 0) jTwiddle w a;
+            let h2 = ST.get() in
+            assert(v (bget h2 jTwiddle 0) = v (bget h1 jTwiddle 0) + (v params_n / (2 * v (bget h1 numoProblems 0))));
+            assert(v (bget h2 jTwiddle 0) < v params_n);
+            numoProblems.(size 0) <- numoProblems.(size 0) >>. size 1
         );
     pop_frame()
 
 /// Inverse NTT implementation only for III-speed and III-size; I has its own which is slightly different.
+
+inline_for_extraction noextract private
+val nttinv_innerfor:
+    numoProblems: size_t{v numoProblems > 0 /\ v numoProblems <= v params_n / 2}
+  -> jFirst: size_t{v jFirst + 2 * v numoProblems < v params_n}
+  -> a: poly
+  -> wj: elem
+  -> Stack size_t
+    (requires fun h -> live h a)
+    (ensures fun h0 _ h1 -> modifies1 a h0 h1)
+
+let nttinv_innerfor numoProblems jFirst a wj = 
+    push_frame();
+    assert(v numoProblems > 0);
+    assert(v jFirst + v numoProblems > v jFirst);
+    assert(v jFirst + v numoProblems = v (jFirst +. numoProblems));
+    let jBuf = create (size 1) jFirst in
+    let liveness h = live h jBuf /\ live h a in
+    let h0 = ST.get() in
+    assert(bget h0 jBuf 0 <. params_n);
+    LL.while
+       (fun h -> liveness h /\ v (bget h jBuf 0) < v params_n /\ modifies2 jBuf a h0 h /\
+              v jFirst + 2 * v numoProblems < v params_n)
+       (fun h -> v (bget h jBuf 0) < v jFirst + v numoProblems)
+       (fun _ -> jBuf.(size 0) <. jFirst +. numoProblems)
+       (fun _ -> 
+           let j:size_t = jBuf.(size 0) in
+           let jNumo = j +. numoProblems in
+           let temp:elem = a.(j) in
+           let ajNumo:elem = a.(jNumo) in
+           assume((v numoProblems <> 16) ==> is_elem (temp +^ ajNumo));
+           assume(FStar.Int.fits (elem_v temp + elem_v ajNumo) elem_n);
+	   if numoProblems = size 16
+	   then ( a.(j) <- barr_reduce ( temp +^ ajNumo ) )
+	   else ( a.(j) <- temp +^ ajNumo );
+           [@inline_let] let difference = temp -^ ajNumo in
+           lemma_elem_product_fits_int64 wj difference;
+           [@inline_let] let product = I64.((elem_to_int64 wj) *^ (elem_to_int64 difference)) in
+           assume(FStar.Int.fits (I64.v product * I64.v params_qinv) I64.n);
+           a.(jNumo) <- reduce product;
+           jBuf.(size 0) <- j +. size 1
+       );
+    let res = jBuf.(size 0) in
+    pop_frame();
+    res
+
+inline_for_extraction noextract private
+val nttinv_middlefor:
+    numoProblems: size_t{v numoProblems > 0 /\ v numoProblems <= v params_n / 2}
+  -> jTwiddle: lbuffer size_t (size 1)
+  -> w: poly
+  -> a: poly
+  -> Stack unit
+    (requires fun h -> live h jTwiddle /\ live h w /\ live h a /\ v (bget h jTwiddle 0) < v params_n)
+    (ensures fun h0 _ h1 -> modifies2 jTwiddle a h0 h1)
+
+let nttinv_middlefor numoProblems jTwiddle w a =
+    push_frame();
+    let jFirst = create (size 1) (size 0) in
+    let cond () : Stack bool
+      (requires fun h -> live h jFirst)
+      (ensures fun h0 _ h1 -> live h1 jFirst)
+    = jFirst.(size 0) <. params_n in
+    let liveness h = live h jTwiddle /\ live h jFirst /\ live h a /\ live h w in
+    let h0 = ST.get() in
+    LL.while // Middle for loop
+        (fun h -> liveness h /\ modifies3 jFirst jTwiddle a h0 h)
+        (fun h -> v (bget h jFirst 0) < v params_n)
+        (fun _ -> jFirst.(size 0) <. params_n)
+        (fun _ ->
+            let jTwiddleVal = jTwiddle.(size 0) in
+            assume(v jTwiddleVal < v params_n);
+            let wj:elem = w.(jTwiddleVal) in
+            jTwiddle.(size 0) <- jTwiddleVal +. (size 1);
+            // TODO (kkane): I *think* j should always be equal to jFirst + numoProblems when it returns, but the
+            // reference code uses j + numoProblems to increment jFirst, and I'm too afraid to deviate
+            // at all from it right now. :)
+            let h = ST.get() in
+            assume(v (bget h jFirst 0) + 2 * v numoProblems < v params_n);
+            let j = nttinv_innerfor numoProblems jFirst.(size 0) a wj in
+            jFirst.(size 0) <- j +. numoProblems
+        );
+    pop_frame()
+    
 val nttinv:
     a: poly
   -> w: poly
@@ -97,59 +251,37 @@ val nttinv:
 
 let nttinv a w =
     push_frame();
-    let numoProblems = create (size 1) (size 1) in
+    let numoProblems:lbuffer size_t (size 1) = create (size 1) (size 1) in
     let jTwiddle = create (size 1) (size 0) in
 
-    while // Outermost for loop
-        #(fun h -> live h numoProblems /\ live h jTwiddle /\ live h a /\ live h w)
-        #(fun _ h -> live h numoProblems /\ live h jTwiddle /\ live h a /\ live h w)
+    let test_pre h = live h numoProblems /\ live h jTwiddle /\ live h a /\ live h w in
+    (*let guard () : Stack bool
+      (requires fun h -> live h numoProblems)
+      (ensures fun h0 _ h1 -> h0 == h1)
+      = numoProblems.(size 0) <. params_n in*)
+
+    let h0 = ST.get() in
+    LL.while // Outermost for loop
+        (fun h -> test_pre h /\ modifies3 numoProblems jTwiddle a h0 h)
+        (fun h -> v (bget h numoProblems 0) < v params_n)
         (fun _ -> numoProblems.(size 0) <. params_n)
         (fun _ ->
-            push_frame();
-            let jBuf = create (size 1) (size 0) in
-            let jFirst = create (size 1) (size 0) in
-            let cond () : Stack bool
-              (requires fun h -> live h jFirst)
-              (ensures fun h0 _ h1 -> live h1 jFirst)
-            = jFirst.(size 0) <. params_n in
-            while // Middle for loop
-                #(fun h -> live h numoProblems /\ live h jTwiddle /\ live h jBuf /\ live h jFirst /\ live h a /\ live h w)
-                #(fun _ h -> live h numoProblems /\ live h jTwiddle /\ live h jBuf /\ live h jFirst /\ live h a /\ live h w)
-                cond
-                (fun _ ->
-                    let jTwiddleVal = jTwiddle.(size 0) in
-                    let wj_elem:elem = w.(jTwiddleVal) in
-                    let wj:sdigit_t = elem_to_sdigit wj_elem in
-                    jTwiddle.(size 0) <- jTwiddleVal +. (size 1);
-                    // Innermost for loop. Have to use a while because the middle for loop's increment depends on the
-                    // final value of j from each inner for loop, so its scope can't be constrained to the for loop.
-                    jBuf.(size 0) <- jFirst.(size 0);
-                    let jFinish = jFirst.(size 0) +. numoProblems.(size 0) in
-                    while
-                        #(fun h -> live h numoProblems /\ live h jTwiddle /\ live h jFirst)
-                        #(fun _ h -> live h numoProblems /\ live h jTwiddle /\ live h jFirst)
-                        (fun _ -> jBuf.(size 0) <. jFinish)
-                        (fun _ ->
-                            let j:size_t = jBuf.(size 0) in
-                            let jNumo = j +. numoProblems.(size 0) in
-                            let temp:elem = a.(j) in
-                            let ajNumo:elem = a.(jNumo) in
-			    if numoProblems.(size 0) = size 16
-			    then ( a.(j) <- barr_reduce ( temp +^ ajNumo ) )
-			    else ( a.(j) <- temp +^ ajNumo );
-                            a.(jNumo) <- reduce I64.((sdigit_to_int64 wj) *^ ((elem_to_int64 temp) -^ (elem_to_int64 ajNumo)));
-			    jBuf.(size 0) <- j +. size 1
-                        );
-                    jFirst.(size 0) <- jBuf.(size 0) +. numoProblems.(size 0)
-                );
-            numoProblems.(size 0) <- numoProblems.(size 0) *. size 2;
-            pop_frame()
+            let h1 = ST.get() in
+            assume(v (bget h1 numoProblems 0) > 0);
+            assume(v (bget h1 numoProblems 0) <= v params_n / 2);
+            assume(v (bget h1 jTwiddle 0) < v params_n);
+            nttinv_middlefor numoProblems.(size 0) jTwiddle w a;
+            numoProblems.(size 0) <- numoProblems.(size 0) *. size 2
         );
 
+    let h1 = ST.get() in
     for 0ul (params_n /. size 2)
-    (fun h _ -> live h a)
+    (fun h _ -> live h a /\ modifies1 a h1 h)
     (fun i ->
+        assert_norm(v params_n / 2 < v params_n);
+        assume(v i < v params_n);
         let ai = a.(i) in
+        assume(FStar.Int.fits (I64.v params_r * elem_v ai * I64.v params_qinv) I64.n); 
 	a.(i) <- reduce I64.(params_r *^ (elem_to_int64 ai))
     );
 
@@ -165,49 +297,78 @@ val poly_pointwise:
 
 let poly_pointwise result x y =
     push_frame();
+    let h0 = ST.get() in
     for (size 0) params_n
-    (fun h _ -> live h result /\ live h x /\ live h y)
+    (fun h _ -> live h result /\ live h x /\ live h y /\ modifies1 result h0 h)
     (fun i ->
         let xi:elem = x.(i) in
         let yi:elem = y.(i) in
+        assume(FStar.Int.fits (elem_v xi * elem_v yi) I64.n);
+        assume(FStar.Int.fits (elem_v xi * elem_v yi * I64.v params_qinv) I64.n);
         result.(i) <- reduce I64.( (elem_to_int64 xi) *^ (elem_to_int64 yi) )
     );
     pop_frame()
+
+#reset-options "--z3rlimit 100 --max_fuel 1 --max_ifuel 1"
 
 val poly_add:
     result: poly
   -> x: poly
   -> y: poly
   -> Stack unit
-    (requires fun h -> live h result /\ live h x /\ live h y /\ disjoint result x /\ disjoint result y /\ disjoint x y)
+    (requires fun h -> live h result /\ live h x /\ live h y /\ disjoint result x /\ disjoint result y /\ disjoint x y /\
+                    (forall i . i < v params_n ==> is_elem_int (elem_v (bget h x i) + elem_v (bget h y i))))
     (ensures fun h0 _ h1 -> modifies1 result h0 h1)
 
 let poly_add result x y =
     push_frame();
+    let h0 = ST.get() in
     for 0ul params_n
-    (fun h _ -> live h result /\ live h x /\ live h y)
+    (fun h _ -> live h result /\ live h x /\ live h y /\ modifies1 result h0 h /\
+             (forall i. i < v params_n ==> is_elem_int (elem_v (bget h x i) + elem_v (bget h y i))))
     (fun i ->
         result.(i) <- x.(i) +^ y.(i)
     );
     pop_frame()
-
+    
 val poly_add_correct:
     result: poly
   -> x: poly
   -> y: poly
   -> Stack unit
-    (requires fun h -> live h result /\ live h x /\ live h y /\ disjoint result x /\ disjoint result y /\ disjoint x y)
+    (requires fun h -> live h result /\ live h x /\ live h y)
     (ensures fun h0 _ h1 -> modifies1 result h0 h1)
 
 let poly_add_correct result x y =
     push_frame();
+    let h0 = ST.get() in
     for 0ul params_n
-    (fun h _ -> live h result /\ live h x /\ live h y)
+    (fun h _ -> live h result /\ live h x /\ live h y /\ modifies1 result h0 h)
     (fun i ->
-        result.(i) <- x.(i) +^ y.(i);
-	result.(i) <- result.(i) +^ ((result.(i) >>^ (size elem_n -. size 1)) &^ params_q);
-	result.(i) <- result.(i) -^ params_q;
-	result.(i) <- result.(i) +^ ((result.(i) >>^ (size elem_n -. size 1)) &^ params_q)
+        let temp:elem_base = x.(i) +^ y.(i) in
+        assert_norm(size elem_n -. size 1 <. size I32.n);
+        assume(elem_v temp >= 0);
+        [@inline_let] let shiftresult = temp >>^ (size elem_n -. size 1) in
+        //assert_norm(elem_v shiftresult == -1 \/ elem_v shiftresult == 0);
+        //assert(elem_v temp < 0 <==> elem_v shiftresult == -1);
+        //assert(elem_v temp >= 0 <==> elem_v shiftresult == 0);
+        [@inline_let] let andresult = shiftresult &^ params_q in
+        //assume(forall (x:elem) . (elem_v (to_elem (-1) &^ x)) == elem_v x);
+        //assert(elem_v temp < 0 ==> elem_v shiftresult == (-1));
+        //assert(elem_v temp < 0 ==> elem_v (shiftresult &^ params_q) == elem_v params_q);
+        //assert(elem_v temp < 0 ==> elem_v andresult == elem_v params_q);
+        //assert(elem_v andresult == elem_v params_q <==> elem_v temp < 0);
+        //assume((elem_v ((to_elem (-1)) &^ params_q)) == elem_v params_q); admit();
+        //assert(elem_v andresult == elem_v params_q \/ elem_v andresult == 0);
+        assume(FStar.Int.fits (elem_v temp + elem_v andresult) I32.n);
+	let temp:elem_base = temp +^ andresult in
+        assume(FStar.Int.fits (elem_v temp - elem_v params_q) I32.n);
+	let temp:elem_base = temp -^ params_q in
+        assume(elem_v temp >= 0);
+        [@inline_let] let addend = ((temp >>^ (size elem_n -. size 1)) &^ params_q) in
+        assume(is_elem_int (elem_v temp + elem_v addend));
+	let temp:elem = temp +^ ((temp >>^ (size elem_n -. size 1)) &^ params_q) in
+        result.(i) <- temp
     );
     pop_frame()
 
@@ -221,11 +382,17 @@ val poly_sub_correct:
 
 let poly_sub_correct result x y =
     push_frame();
+    let h0 = ST.get() in
     for 0ul params_n
-    (fun h _ -> live h result /\ live h x /\ live h y)
+    (fun h _ -> live h result /\ live h x /\ live h y /\ modifies1 result h0 h)
     (fun i ->
-        result.(i) <- x.(i) -^ y.(i);
-	result.(i) <- result.(i) +^ ((result.(i) >>^ (size elem_n -. size 1)) &^ params_q)
+        let temp:elem_base = x.(i) -^ y.(i) in
+        assert_norm(size elem_n -. size 1 <. size I32.n);
+        assume(elem_v temp >= 0);
+        assume(FStar.Int.fits (elem_v temp + elem_v ((temp >>^ (size elem_n -. size 1)) &^ params_q)) elem_n);
+        let temp:elem_base = temp +^ ((temp >>^ (size elem_n -. size 1)) &^ params_q) in
+        assume(is_elem temp);
+        result.(i) <- temp
     );
     pop_frame()
 
@@ -234,16 +401,18 @@ val poly_sub_reduce:
   -> x: poly
   -> y: poly
   -> Stack unit
-    (requires fun h -> live h result /\ live h x /\ live h y)
+    (requires fun h -> live h result /\ live h x /\ live h y /\ disjoint result x /\ disjoint result y)
     (ensures fun h0 _ h1 -> modifies1 result h0 h1)
 
 let poly_sub_reduce result x y =
     push_frame();
+    let h0 = ST.get() in
     for 0ul params_n
-    (fun h _ -> live h result /\ live h x /\ live h y)
+    (fun h _ -> live h result /\ live h x /\ live h y /\ modifies1 result h0 h)
     (fun i ->
         let xi = x.(i) in
         let yi = y.(i) in
+        assume(FStar.Int.fits (I64.v params_r * (elem_v xi - elem_v yi) * I64.v params_qinv) I64.n);
         result.(i) <- reduce I64.(params_r *^ ((elem_to_int64 xi) -^ (elem_to_int64 yi)))
     );
     pop_frame()
