qtesla/code/Hacl.Impl.QTesla.Lemmas.fst
@@ -27,6 +27,14 @@ val lemma_logand32_value_min: x:I64.t -> Lemma
 
 let lemma_logand32_value_min _ = admit()
 
+val elem_product_fits_int64: x:elem_base -> y:elem_base -> GTot bool
+let elem_product_fits_int64 x y = FStar.Int.fits (elem_v x * elem_v y) 64
+
+val lemma_elem_product_fits_int64: x:elem_base -> y:elem_base -> Lemma
+  (ensures elem_product_fits_int64 x y /\ FStar.Int.fits (elem_v x * elem_v y * I64.v params_qinv) 64)
+
+let lemma_elem_product_fits_int64 x y = admit()
+
 (*
 val lemma_logand_value_max: x:I64.t -> n:nat -> Lemma
   (requires (n >= 2 /\ n <= 64 /\ FStar.Int.fits (pow2 n - 1) n))
