qtesla/code/Hacl.Impl.QTesla.fst
@@ -23,6 +23,7 @@ open Lib.Buffer
 open Lib.ByteBuffer
 
 open C.Loops
+module LL = Lib.Loops
 
 open Hacl.Impl.QTesla.Params
 open Hacl.Impl.QTesla.Platform
@@ -44,7 +45,7 @@ module SHA3 = Hacl.SHA3
 
 module R    = Hacl.QTesla.Random
 
-#reset-options "--z3rlimit 100 --max_fuel 0 --max_ifuel 0 --admit_smt_queries true"
+#reset-options "--z3rlimit 100 --max_fuel 1 --max_ifuel 1"
 
 private let _RADIX32 = size params_radix32
 
@@ -52,9 +53,11 @@ private let _RADIX32 = size params_radix32
 // it's important to do this. In one case the return value is compared against a quantity that isn't even close
 // to exceeding the maximum value of a signed int32, much less an int64, and in all other cases ends up getting
 // immediately cast back into a signed type.
-val abs_: value: I32.t -> Tot (x:I32.t{I32.(x >=^ 0l)})
+val abs_: value: I32.t -> Tot I32.t
 let abs_ value = 
+    assert_norm(v (_RADIX32 -. size 1) < I32.n);
     let mask = I32.(value >>^ (_RADIX32 -. size 1)) in
+    assume(FStar.Int.fits (elem_v (mask ^^ value) - elem_v mask) I32.n);
     I32.((mask ^^ value) -^ mask)
 
 val check_ES:
@@ -62,7 +65,7 @@ val check_ES:
   -> bound: UI32.t
   -> Stack bool
     (requires fun h -> live h p)
-    (ensures fun h0 _ h1 -> h0 == h1)
+    (ensures fun h0 _ h1 -> modifies0 h0 h1)
 
 let check_ES p bound =
   push_frame();
@@ -82,31 +85,45 @@ let check_ES p bound =
   let temp = create (size 1) 0l in
   let mask = create (size 1) 0l in
   let list = create params_n 0l in
+  let h0 = ST.get () in
   for (size 0) params_n
-      (fun h _ -> live h p /\ live h list)
+      (fun h _ -> live h p /\ live h list /\ modifies1 list h0 h)
       (fun j ->
         let pj = p.(j) in
         let abspj = abs_ (elem_to_int32 pj) in
         list.(j) <- abspj
       );
 
+  let h1 = ST.get () in
   for (size 0) params_h
-      (fun h _ -> live h p /\ live h sum /\ live h limit /\ live h temp /\ live h mask /\ live h list)
+      (fun h _ -> live h p /\ live h sum /\ live h limit /\ live h temp /\ live h mask /\ live h list /\
+               modifies (loc mask |+| loc temp |+| loc list |+| loc sum |+| loc limit) h1 h /\
+               v (bget h limit 0) <= v params_n)
       (fun j ->
           let loopMax = (limit.(size 0)) -. size 1 in
+          let h2 = ST.get () in
           for 0ul loopMax
-          (fun h _ -> live h p /\ live h sum /\ live h limit /\ live h temp /\ live h mask /\ live h list)
+          (fun h _ -> live h p /\ live h sum /\ live h limit /\ live h temp /\ live h mask /\ live h list /\
+                   modifies3 mask temp list h2 h /\ v (bget h limit 0) <= v params_n)
           (fun i ->
+              let h3 = ST.get () in
+              assume(v i < v params_n - 1);
+              assume(FStar.Int.fits (I32.v (bget h3 list (v i + 1)) - I32.v (bget h3 list (v i))) I32.n);
+              assert_norm(v (_RADIX32 -. size 1) < 32);
               mask.(size 0) <- ((list.(i +. size 1)) -^ (list.(i))) >>^ (_RADIX32 -. size 1);
               temp.(size 0) <- ((list.(i +. size 1)) &^ (mask.(size 0))) |^
                                     ((list.(i)) &^ (lognot mask.(size 0)));
               list.(i +. size 1) <- (list.(i)) &^ mask.(size 0) |^
                                    (list.(i +. (size 1))) &^ (lognot mask.(size 0));
               list.(i) <- temp.(size 0)
-          );
+          ); 
 
           let listIndex = limit.(size 0) -. size 1 in
+          let h4 = ST.get () in
+          assume(v ((bget h4 limit 0) -. size 1) < v params_n);
           let listAmt = list.(listIndex) in
+          let h5 = ST.get () in
+          assume(FStar.UInt.fits (UI32.v (bget h5 sum 0) + UI32.v (int32_to_uint32 listAmt)) UI32.n);
           sum.(size 0) <- UI32.(sum.(size 0) +^ int32_to_uint32 listAmt);
           limit.(size 0) <- limit.(size 0) -. size 1
       );
@@ -116,7 +133,52 @@ let check_ES p bound =
    pop_frame();
    res
 
-open Lib.ByteBuffer
+#reset-options "--z3rlimit 300 --max_fuel 1 --max_ifuel 1"// --print_z3_statistics --log_queries --query_stats"
+
+private inline_for_extraction noextract
+val poly_uniform_valFromBuffer:
+    pos: lbuffer size_t (size 1)
+  -> buf: lbuffer uint8 (shake128_rate *. params_genA)
+  -> mask: uint32
+  -> Stack pub_uint32
+    (requires fun h -> live h pos /\ live h buf /\ disjoint pos buf /\
+                    v (bget h pos 0) + numbytes U32 <= v (shake128_rate *. params_genA))
+    (ensures fun h0 _ h1 -> modifies2 pos buf h0 h1)
+
+let poly_uniform_valFromBuffer pos buf mask =
+    push_frame();
+    let nbytes:size_t = (params_q_log +. 7ul) /. 8ul in    
+    let pos0 = pos.(size 0) in
+    let subbuff = sub buf pos0 (size (numbytes U32)) in
+    let bufPosAsUint:uint32 = uint_from_bytes_le subbuff in
+    let val1:uint32 = bufPosAsUint &. mask in
+    pos.(size 0) <- pos0 +. nbytes;
+    pop_frame();
+    // It is safe to compare this value with the regular less-than operator, so we declassify it to do that.
+    unsafe_declassify val1
+
+private inline_for_extraction noextract
+val poly_uniform_setA:
+    a: poly
+  -> iBuf: lbuffer size_t (size 1)
+  -> value: pub_uint32
+  -> Stack unit
+    (requires fun h -> live h a /\ live h iBuf /\ disjoint a iBuf /\
+                    ((v value < elem_v params_q /\ v (bget h iBuf 0) < (v params_k * v params_n)) ==>
+                    FStar.Int.fits (v value * I64.v params_r2_invn * I64.v params_qinv) I64.n))
+    (ensures fun h0 _ h1 -> modifies2 a iBuf h0 h1 /\ 
+                         ((v value < elem_v params_q /\ v (bget h0 iBuf 0) < (v params_k * v params_n)) ==>
+                          v (bget h1 iBuf 0) = v (bget h0 iBuf 0) + 1))
+
+let poly_uniform_setA a iBuf value =
+    push_frame();
+    [@inline_let] let params_q = elem_to_uint32 params_q in
+    let i = iBuf.(size 0) in
+    if (value <. params_q && i <. (params_k *. params_n))
+    then ( a.(i) <- reduce I64.((uint32_to_int64 value) *^ params_r2_invn);
+           iBuf.(size 0) <- i +. size 1 )
+    else ();
+    pop_frame()
 
 val poly_uniform:
     a: poly
@@ -124,161 +186,191 @@ val poly_uniform:
   -> Stack unit
     (requires fun h -> live h a /\ live h seed /\ disjoint a seed)
     (ensures fun h0 _ h1 -> modifies1 a h0 h1)
-
+    
 let poly_uniform a seed =
     push_frame();
     let pos = create (size 1) (size 0) in
-    let i = create (size 1) (u32 0) in
+    let i = create (size 1) (size 0) in
     let nbytes:size_t = (params_q_log +. 7ul) /. 8ul in
     let nblocks = create (size 1) params_genA in
-    let mask:UI32.t = UI32.((1ul <<^ params_q_log) -^ 1ul) in
+    let mask:uint32 = (u32 1 <<. params_q_log) -. u32 1 in
     let buf = create (shake128_rate *. params_genA) (u8 0) in
-    let dmsp = create (size 1) 0us in
+    let dmsp = create (size 1) (u16 0) in
     cshake128_qtesla crypto_randombytes seed (dmsp.(size 0)) (shake128_rate *. params_genA) buf;
-    dmsp.(size 0) <- UI16.((dmsp.(size 0)) +^ 1us);
+    dmsp.(size 0) <- dmsp.(size 0) +. (u16 1);
 
-    while
-        #(fun h -> live h pos /\ live h i /\ live h nblocks /\ live h buf /\ live h dmsp)
-        #(fun _ h -> live h pos /\ live h i /\ live h nblocks /\ live h buf /\ live h dmsp)
-        ( fun _ -> (i.(size 0)) <. (params_k *. params_n) )
-        ( fun _ ->
+    let h0 = ST.get () in
+    LL.while
+        (fun h -> live h a /\ live h pos /\ live h i /\ live h nblocks /\ live h buf /\ live h dmsp /\ live h seed /\
+               modifies (loc dmsp |+| loc pos |+| loc a |+| loc i |+| loc nblocks |+| loc buf) h0 h)
+        (fun h -> v (bget h i 0) < v params_k * v params_n)
+        (fun _ -> i.(size 0) <. (params_k *. params_n) )
+        (fun _ ->
             if (pos.(size 0)) >. (shake128_rate *. (nblocks.(size 0))) -. ((size 4) *. nbytes)
-            then ( nblocks.(size 0) <- 1ul;
-	         let bufSize:size_t = shake128_rate *. (nblocks.(size 0)) in
-                 cshake128_qtesla crypto_randombytes seed (dmsp.(size 0)) (bufSize) buf;
-                 dmsp.(size 0) <- UI16.((dmsp.(size 0)) +^ 1us);
-                 pos.(size 0) <- 0ul )
+            then ( nblocks.(size 0) <- size 1;
+	         let bufSize:size_t = shake128_rate *. nblocks.(size 0) in
+                 let subbuff = sub buf (size 0) bufSize in
+                 cshake128_qtesla crypto_randombytes seed dmsp.(size 0) bufSize subbuff;
+                 dmsp.(size 0) <- dmsp.(size 0) +. u16 1;
+                 pos.(size 0) <- size 0 )
             else ();
-
+(*
             let bufSize:size_t = (nblocks.(size 0)) *. shake128_rate in
 
             let pos0 = pos.(size 0) in
+            assume(v pos0 + numbytes U32 <= v (shake128_rate *. params_genA));
             let subbuff = sub buf pos0 (size (numbytes U32)) in
-            let bufPosAsUint = uint_from_bytes_le #U32 #PUB subbuff in
-            let val1 = bufPosAsUint &. mask in
-            pos.(size 0) <- UI32.(pos0 +^ nbytes);
+            let bufPosAsUint:uint32 = uint_from_bytes_le subbuff in
+            let val1:uint32 = bufPosAsUint &. mask in
+            pos.(size 0) <- pos0 +. nbytes;
 
             let pos0 = pos.(size 0) in
+            assume(v pos0 + numbytes U32 <= v (shake128_rate *. params_genA));
             let subbuff = sub buf pos0 (size (numbytes U32)) in
-            let bufPosAsUint = uint_from_bytes_le #U32 #PUB subbuff in
-            let val2 = bufPosAsUint &. mask in
-            pos.(size 0) <- UI32.(pos0 +^ nbytes);
-            
-            let pos0 = pos.(size 0) in
-            let subbuff = sub buf pos0 (size (numbytes U32)) in
-            let bufPosAsUint = uint_from_bytes_le #U32 #PUB subbuff in
-            let val3 = bufPosAsUint &. mask in
-            pos.(size 0) <- UI32.(pos0 +^ nbytes);
+            let bufPosAsUint:uint32 = uint_from_bytes_le subbuff in
+            let val2:uint32 = bufPosAsUint &. mask in
+            pos.(size 0) <- pos0 +. nbytes;
 
             let pos0 = pos.(size 0) in
+            assume(v pos0 + numbytes U32 <= v (shake128_rate *. params_genA));
             let subbuff = sub buf pos0 (size (numbytes U32)) in
-            let bufPosAsUint = uint_from_bytes_le #U32 #PUB subbuff in
-            let val4 = bufPosAsUint &. mask in
-            pos.(size 0) <- UI32.(pos0 +^ nbytes);
+            let bufPosAsUint:uint32 = uint_from_bytes_le subbuff in
+            let val3:uint32 = bufPosAsUint &. mask in
+            pos.(size 0) <- pos0 +. nbytes;
 
-            if (let iVal = i.(size 0) in val1 <. params_q && iVal <. (params_k *. params_n))
-            then ( a.(i.(size 0)) <- reduce I64.((uint32_to_int64 val1) *^ params_r2_invn);
-                 i.(size 0) <- UI32.((i.(size 0)) +^ 1ul) )
+            let pos0 = pos.(size 0) in
+            assume(v pos0 + numbytes U32 <= v (shake128_rate *. params_genA));
+            let subbuff = sub buf pos0 (size (numbytes U32)) in
+            let bufPosAsUint:uint32 = uint_from_bytes_le subbuff in
+            let val4:uint32 = bufPosAsUint &. mask in
+            pos.(size 0) <- pos0 +. nbytes;            
+*)
+
+            let h1 = ST.get () in assume(v (bget h1 pos 0) + numbytes U32 <= v (shake128_rate *. params_genA));
+            let val1 = poly_uniform_valFromBuffer pos buf mask in
+            let h1 = ST.get () in assume(v (bget h1 pos 0) + numbytes U32 <= v (shake128_rate *. params_genA));
+            let val2 = poly_uniform_valFromBuffer pos buf mask in
+            let h1 = ST.get () in assume(v (bget h1 pos 0) + numbytes U32 <= v (shake128_rate *. params_genA));
+            let val3 = poly_uniform_valFromBuffer pos buf mask in
+            let h1 = ST.get () in assume(v (bget h1 pos 0) + numbytes U32 <= v (shake128_rate *. params_genA));
+            let val4 = poly_uniform_valFromBuffer pos buf mask in
+
+            (*[@inline_let] let params_q = elem_to_uint32 params_q in
+            let iVal = i.(size 0) in
+            if (val1 <. params_q && iVal <. (params_k *. params_n))
+            then ( assume(FStar.Int.fits (UI32.v val1 * I64.v params_r2_invn * Int64.v params_qinv) I64.n);
+                   a.(iVal) <- reduce I64.((uint32_to_int64 val1) *^ params_r2_invn);
+                   i.(size 0) <- iVal +. size 1 )
+            else (); 
+            let iVal = i.(size 0) in
+            if (val2 <. params_q && iVal <. (params_k *. params_n))
+            then ( assume(FStar.Int.fits (UI32.v val2 * I64.v params_r2_invn * Int64.v params_qinv) I64.n);
+                   a.(iVal) <- reduce I64.((uint32_to_int64 val2) *^ params_r2_invn);
+                   i.(size 0) <- iVal +. size 1 )
             else ();
-            if (let iVal = i.(size 0) in val2 <. params_q && iVal <. (params_k *. params_n))
-            then ( a.(i.(size 0)) <- reduce I64.((uint32_to_int64 val2) *^ params_r2_invn);
-                 i.(size 0) <- UI32.((i.(size 0)) +^ 1ul) )
+            let iVal = i.(size 0) in
+            if (val3 <. params_q && iVal <. (params_k *. params_n))
+            then ( assume(FStar.Int.fits (UI32.v val3 * I64.v params_r2_invn * Int64.v params_qinv) I64.n);
+                   a.(iVal) <- reduce I64.((uint32_to_int64 val3) *^ params_r2_invn);
+                   i.(size 0) <- iVal +. size 1 )
             else ();
-            if (let iVal = i.(size 0) in val3 <. params_q && iVal <. (params_k *. params_n))
-            then ( a.(i.(size 0)) <- reduce I64.((uint32_to_int64 val3) *^ params_r2_invn);
-                 i.(size 0) <- UI32.((i.(size 0)) +^ 1ul) )
-            else ();
-            if (let iVal = i.(size 0) in val4 <. params_q && iVal <. (params_k *. params_n))
-            then ( a.(i.(size 0)) <- reduce I64.((uint32_to_int64 val4) *^ params_r2_invn);
-                 i.(size 0) <- UI32.((i.(size 0)) +^ 1ul) )
-            else ()
+            let iVal = i.(size 0) in
+            if (val4 <. params_q && iVal <. (params_k *. params_n))
+            then ( assume(FStar.Int.fits (UI32.v val4 * I64.v params_r2_invn * Int64.v params_qinv) I64.n);
+                   a.(iVal) <- reduce I64.((uint32_to_int64 val4) *^ params_r2_invn);
+                   i.(size 0) <- iVal +. size 1 )
+            else ()*)
+
+            assume(FStar.Int.fits (UI32.v val1 * I64.v params_r2_invn * Int64.v params_qinv) I64.n);
+            poly_uniform_setA a i val1;
+            assume(FStar.Int.fits (UI32.v val2 * I64.v params_r2_invn * Int64.v params_qinv) I64.n);
+            poly_uniform_setA a i val2;
+            assume(FStar.Int.fits (UI32.v val3 * I64.v params_r2_invn * Int64.v params_qinv) I64.n);
+            poly_uniform_setA a i val3;
+            assume(FStar.Int.fits (UI32.v val4 * I64.v params_r2_invn * Int64.v params_qinv) I64.n);
+            poly_uniform_setA a i val4
         );
 
     pop_frame()
 
-val qtesla_keygen:
-    pk: buffer uint8
-  -> sk: buffer uint8
-  -> Stack I32.t
-    (requires fun h -> live h pk /\ live h sk /\ disjoint pk sk)
-    (ensures fun h0 _ h1 -> modifies (loc pk |+| loc sk) h0 h1)
+#reset-options "--z3rlimit 100 --max_fuel 0 --max_ifuel 0"
 
-// Preliminary work using one of Santiago's loop combinators for the first for loop
-(*assume val keygen_sample_spec:
-    #rlen:size_nat
-  -> rand:Lib.ByteSequence.lbytes rlen
-  -> nonce:nat
-  -> i:size_nat
-  -> e:LibSeq.lseq poly (v params_k)
-  -> Tot (LibSeq.lseq poly (v params_k))*)
-//let keygen_sample_spec #rlen rand nonce i e ="*)
-
-  (*[@inline_let]
-  let spec h0 = keygen_sample_spec (as_seq h0 randomness_extended) (get h0 nonce 0) in
-  loop1 h0 (size params_k) e spec
-  (fun k ->
-    C.Loops.do_while
-      (fun h stop -> live h e /\ live h randomness_extended /\
-                   (not stop ==> (check_ES (get h e k) params_Le)) /\
-                   (stop ==> (not (check_ES (get h e k) params_Le))))
-      (fun _ ->
-        let nonce0 = nonce.(size 0) in
-        nonce.(size 0) <- nonce0 +. 1;
-        sample_gauss_poly e.(k) (sub randomness_extended (k * crypto_seedbytes) crypto_randombytes) nonce;
-        not (check_ES e.(k) params_Le)));*)
-
-inline_for_extraction noextract private
+private inline_for_extraction noextract
 let randomness_extended_size = (params_k +. size 3) *. crypto_seedbytes
 
-let qtesla_keygen pk sk =
+private inline_for_extraction noextract
+val qtesla_keygen_sample_gauss_poly:
+    randomness_extended: lbuffer uint8 randomness_extended_size
+  -> nonce: lbuffer uint32 (size 1)
+  -> p: poly
+  -> k: size_t{v k <= v params_k}
+  -> Stack unit
+    (requires fun h -> live h randomness_extended /\ live h nonce /\ live h p /\ 
+                    disjoint randomness_extended nonce /\ disjoint randomness_extended p /\ disjoint nonce p)
+    (ensures fun h0 _ h1 -> modifies2 nonce p h0 h1)
+
+let qtesla_keygen_sample_gauss_poly randomness_extended nonce p k =
+    let subbuffer = sub randomness_extended (k *. crypto_seedbytes) crypto_randombytes in
+    let nonce0 = nonce.(size 0) in
+    nonce.(size 0) <- nonce0 +. u32 1;
+    let nonce1 = nonce.(size 0) in
+    sample_gauss_poly p subbuffer nonce1
+
+(*let test (e:poly_k) (k:size_t{v k < v params_k}) : Stack unit (requires fun h -> live h e) (ensures fun _ _ _ -> True) =
+    //let ek = sub e (k *. params_n) params_n in
+    let ek2 = index_poly e k in
+    //assert(loc_includes (loc e) (loc ek));
+    assert(loc_includes (loc e) (loc ek2))*)
+
+private inline_for_extraction noextract
+val qtesla_keygen_:
+    randomness: lbuffer uint8 crypto_randombytes
+  -> pk: lbuffer uint8 crypto_publickeybytes
+  -> sk: lbuffer uint8 crypto_secretkeybytes
+  -> Stack (r:I32.t{r == 0l})
+    (requires fun h -> live h randomness /\ live h pk /\ live h sk /\ 
+                    disjoint randomness pk /\ disjoint randomness sk /\ disjoint pk sk)
+    (ensures fun h0 _ h1 -> modifies2 pk sk h0 h1)
+
+#reset-options "--z3rlimit 300 --max_fuel 0 --max_ifuel 0 --z3cliopt 'smt.qi.eager_threshold=100'"
+let qtesla_keygen_ randomness pk sk =
   push_frame();
-  let randomness = create crypto_randombytes (u8 0) in
   let randomness_extended = create randomness_extended_size (u8 0) in
   let e:poly_k = poly_k_create () in
   let s:poly = poly_create () in
   let s_ntt:poly = poly_create () in
   let a:poly_k = poly_k_create () in
   let t:poly_k = poly_k_create () in 
-  let nonce = create (size 1) 0L in
-  R.randombytes_ crypto_randombytes randomness;
+  let nonce = create (size 1) (u32 0) in
   params_SHAKE crypto_randombytes randomness randomness_extended_size randomness_extended;
-
+  let h0 = ST.get () in
   for (size 0) params_k
-      (fun h _ -> live h nonce /\ live h e /\ live h randomness_extended)
+      (fun h _ -> live h nonce /\ live h e /\ live h randomness_extended /\ modifies2 nonce e h0 h)
       (fun k ->
         do_while
-          (fun h stop -> live h nonce /\ live h e /\ live h randomness_extended)
-                       //(stop ==> (not (check_ES (get_poly e k) params_Le))))
+          (fun h _ -> live h nonce /\ live h e /\ live h randomness_extended /\ modifies2 nonce e h0 h)
           (fun _ ->
-            let subbuffer = sub randomness_extended (k *. crypto_seedbytes) crypto_randombytes in
-            let nonce0 = nonce.(size 0) in
-            nonce.(size 0) <- I64.(nonce0 +^ 1L);
-            let nonce1:uint64 = nonce.(size 0) in
-            let ek:poly = index_poly e k in
-            sample_gauss_poly ek subbuffer nonce1;
-            // TODO: ek is a buffer, and so we shouldn't have to refetch it with index_poly to operate on its current value, right?
+            let ek = index_poly e k in
+            qtesla_keygen_sample_gauss_poly randomness_extended nonce ek k;
             not (check_ES ek params_Le)
           )
-      );
+      ); 
+  let h1 = ST.get () in
   do_while
-      (fun h stop -> live h s /\ live h randomness_extended /\ live h nonce)
-                   //(stop ==> (not (check_ES s params_Ls)))) // TODO: need Ghost/Tot version of check_ES for invariants
+      (fun h stop -> live h s /\ live h randomness_extended /\ live h nonce /\ modifies2 nonce s h1 h)
       (fun _ ->
-        let rndsubbuffer = sub randomness_extended (params_k *. crypto_seedbytes) crypto_randombytes in
-        let nonce0:uint64 = nonce.(size 0) in
-        nonce.(size 0) <- nonce0 +. (u64 1);
-        let nonce1:uint64 = nonce.(size 0) in
-        sample_gauss_poly s rndsubbuffer nonce1;
+        qtesla_keygen_sample_gauss_poly randomness_extended nonce s params_k;
         not (check_ES s params_Ls)
-      );
-
-  let rndsubbuffer = sub randomness_extended ((params_k +. (size 1)) *. crypto_seedbytes) crypto_randombytes in
-  poly_uniform a rndsubbuffer;
+      ); 
+  let h2 = ST.get () in
+  let rndsubbuffer = sub randomness_extended ((params_k +. (size 1)) *. crypto_seedbytes) (size 2 *. crypto_seedbytes) in
+  poly_uniform a (sub rndsubbuffer (size 0) crypto_randombytes);
+  let h3 = ST.get () in
 
   poly_ntt s_ntt s;
-
+  let h4 = ST.get () in
   C.Loops.for (size 0) params_k
-      (fun h _ -> live h t /\ live h a /\ live h s_ntt /\ live h e)
+      (fun h _ -> live h t /\ live h a /\ live h s_ntt /\ live h e /\ modifies1 t h4 h)
       (fun k ->
           let tk:poly = index_poly t k in
           let ak:poly = index_poly a k in
@@ -287,11 +379,32 @@ let qtesla_keygen pk sk =
           poly_add_correct tk tk ek
         );
 
+  let h5 = ST.get () in
   encode_or_pack_sk sk s e rndsubbuffer;
-  encode_pk pk t rndsubbuffer;
-
-  pop_frame();
+  let h6 = ST.get () in
+  encode_pk pk t (sub rndsubbuffer (size 0) crypto_seedbytes);
+  let h7 = ST.get () in
+  pop_frame(); //admit();
   0l
+
+#reset-options "--z3rlimit 100 --max_fuel 0 --max_ifuel 0"
+
+val qtesla_keygen:
+    pk: lbuffer uint8 crypto_publickeybytes
+  -> sk: lbuffer uint8 crypto_secretkeybytes
+  -> Stack (r:I32.t{r == 0l})
+    (requires fun h -> live h pk /\ live h sk /\ 
+                    disjoint R.state pk /\ disjoint R.state sk /\ disjoint pk sk)
+    (ensures fun h0 _ h1 -> modifies3 R.state pk sk h0 h1)
+
+let qtesla_keygen pk sk =
+    recall R.state;
+    push_frame();
+    let randomness = create crypto_randombytes (u8 0) in
+    R.randombytes_ crypto_randombytes randomness;
+    let r = qtesla_keygen_ randomness pk sk in
+    pop_frame();
+    r
 
 val sample_y:
     y : poly
@@ -312,31 +425,43 @@ let sample_y y seed nonce =
     let nblocks = create (size 1) params_n in
     let buf = create (params_n *. bplus1bytes ) (u8 0) in
     let nbytes = bplus1bytes in
-    let dmsp:(lbuffer UI16.t (size 1)) = create (size 1) (int32_to_uint16 I32.(nonce <<^ 8ul)) in
+    [@inline_let] let dmspVal:uint16 = cast U16 SEC (Lib.RawIntTypes.u16_from_UInt16 (int32_to_uint16 I32.(nonce <<^ 8ul))) in
+    let dmsp = create (size 1) dmspVal in
 
     params_cSHAKE crypto_randombytes seed dmsp.(size 0) (params_n *. nbytes) buf;
-    dmsp.(size 0) <- UI16.(dmsp.(size 0) +^ 1us);
+    let hInit = ST.get () in
+    assume(v (bget hInit dmsp 0) < pow2 ((bits U16) - 1));
+    dmsp.(size 0) <- dmsp.(size 0) +. u16 1;
 
-    while
-    #(fun h -> live h y /\ live h i /\ live h pos /\ live h nblocks /\ live h buf /\ live h dmsp)
-    #(fun _ h -> live h y /\ live h i /\ live h pos /\ live h nblocks /\ live h buf /\ live h dmsp)
+    let h0 = ST.get () in
+    LL.while
+    (fun h -> live h y /\ live h i /\ live h pos /\ live h nblocks /\ live h buf /\ live h dmsp /\
+           modifies (loc y |+| loc i |+| loc pos |+| loc nblocks |+| loc buf |+| loc dmsp) h0 h)
+    (fun h -> v (bget h i 0) < v params_n)
     (fun _ -> i.(size 0) <. params_n)
     (fun _ ->
         if pos.(size 0) >=. nblocks.(size 0) *. nbytes
 	then (
 	    nblocks.(size 0) <- nblocks_shake;
-	    params_cSHAKE crypto_randombytes seed dmsp.(size 0) shake_rate buf;
-	    dmsp.(size 0) <- UI16.(dmsp.(size 0) +^ 1us);
+	    params_cSHAKE crypto_randombytes seed dmsp.(size 0) shake_rate (sub buf (size 0) shake_rate);
+            assume(v (bget hInit dmsp 0) < pow2 ((bits U16) - 1));
+	    dmsp.(size 0) <- dmsp.(size 0) +. u16 1;
 	    pos.(size 0) <- size 0
 	) else ();
 
         let pos0 = pos.(size 0) in
+        assume(v pos0 + numbytes U32 <= v (params_n *. bplus1bytes));
 	let subbuff = sub buf pos0 (size (numbytes U32)) in
-	let bufPosAsU32 = uint_from_bytes_le #U32 #PUB subbuff in
-	let bufPosAsElem = uint32_to_elem bufPosAsU32 in
+	let bufPosAsU32 = uint_from_bytes_le #U32 #_ subbuff in
+	let bufPosAsElem = uint32_to_elem (Lib.RawIntTypes.u32_to_UInt32 bufPosAsU32) in
 	let i0 = i.(size 0) in
 	// Heuristic parameter sets do four at once. Perf. But optional.
+        let h1 = ST.get () in
+        assume(FStar.Int.fits (elem_v (to_elem 1 <<^ (params_b_bits +. size 1)) - 1) elem_n);
+        assume(is_elem (bufPosAsElem &^ ((to_elem 1 <<^ (params_b_bits +. size 1)) -^ to_elem 1)));
 	y.(i0) <- bufPosAsElem &^ ((to_elem 1 <<^ (params_b_bits +. size 1)) -^ to_elem 1);
+        let h2 = ST.get () in
+        assume(is_elem ((bget h2 y (v i0)) -^ params_B));
 	y.(i0) <- y.(i0) -^ params_B;
 	if y.(i0) <> (to_elem 1 <<^ params_b_bits)
 	then ( i.(size 0) <- i0 +. size 1 )
@@ -346,42 +471,52 @@ let sample_y y seed nonce =
 
     pop_frame()
     
-
 val hash_H:
-    c_bin : buffer uint8
+    c_bin : lbuffer uint8 crypto_c_bytes
   -> v : poly_k
-  -> hm : buffer uint8
+  -> hm : lbuffer uint8 crypto_hmbytes
   -> Stack unit
     (requires fun h -> live h c_bin /\ live h v /\ live h hm /\ disjoint c_bin v /\ disjoint c_bin hm /\ disjoint v hm)
-    (ensures fun h0 _ h1 -> live h1 c_bin /\ live h1 v /\ live h1 hm /\ modifies (loc c_bin) h0 h1)
+    (ensures fun h0 _ h1 -> modifies1 c_bin h0 h1)
 
 let hash_H c_bin v_ hm =
     push_frame();
 
     [@inline_let] let params_q = elem_to_int32 params_q in
     let t = create (params_k *. params_n +. crypto_hmbytes) (u8 0) in
-    let index = create (size 1) (size 0) in
 
+    let h0 = ST.get () in
     for 0ul params_k
-    (fun h _ -> live h c_bin /\ live h v_ /\ live h hm)
+    (fun h _ -> live h v_ /\ live h t /\ modifies1 t h0 h)
     (fun k ->
-        index.(size 0) <- k *. params_n;
+        push_frame();
+        let index = create (size 1) (k *. params_n) in
+        let h1 = ST.get () in
 	for 0ul params_n
-	(fun h _ -> live h c_bin /\ live h v_ /\ live h hm /\ live h index)
+	(fun h i -> live h v_ /\ live h t /\ live h index /\ modifies2 t index h1 h) ///\ 
+                 //(i < v params_n ==> v (bget h index 0) < v (k *. params_n +. params_n)))
 	(fun i ->
 	    let vindex:elem = v_.(index.(size 0)) in
 	    let temp:I32.t = elem_to_int32 vindex in
+            assert_norm(v (_RADIX32 -. size 1) < I32.n);
 	    let mask = I32.((params_q /^ 2l -^ temp) >>^ (_RADIX32 -. size 1)) in
 	    let temp = I32.(((temp -^ params_q) &^ mask) |^ (temp &^ (lognot mask))) in
+            assume(FStar.Int.fits (I32.v (1l <<^ params_d) - 1) I32.n);
 	    let cL = I32.(temp &^ ((1l <<^ params_d) -^ 1l)) in
+            assert_norm(v (params_d -. size 1) < I32.n);
+            assume(FStar.Int.fits (I32.v ((1l <<^ (params_d -. (size 1)))) - I32.v cL) I32.n);
 	    let mask = I32.(((1l <<^ (params_d -. (size 1))) -^ cL) >>^ (_RADIX32 -. size 1)) in
+            assume(FStar.Int.fits (I32.v cL - (I32.v (1l <<^ params_d))) I32.n);
 	    let cL = I32.(((cL -^ (1l <<^ params_d)) &^ mask) |^ (cL &^ (lognot mask))) in
-	    t.(index.(size 0)) <- int32_to_uint8 I32.((temp -^ cL) >>^ params_d);
+            assume(FStar.Int.fits (I32.v temp - I32.v cL) I32.n);
+	    t.(index.(size 0)) <- Lib.RawIntTypes.u8_from_UInt8 (int32_to_uint8 I32.((temp -^ cL) >>^ params_d));
 	    // Putting (index.(size 0)) inline in the assignment causes a typing error for some reason.
 	    // Opened a bug on this.
 	    let indexVal:size_t = index.(size 0) in
+            assume(v indexVal + 1 < v (k *. params_n +. params_n));
 	    index.(size 0) <- indexVal +. (size 1)
-	)
+	);
+        pop_frame()
     );
 
     update_sub #MUT #_ #_ t (params_k *. params_n) crypto_hmbytes hm;
@@ -392,11 +527,13 @@ let hash_H c_bin v_ hm =
 val encode_c:
     pos_list : lbuffer UI32.t params_h
   -> sign_list : lbuffer I16.t params_h
-  -> c_bin : buffer uint8
+  -> c_bin : lbuffer uint8 crypto_c_bytes
   -> Stack unit
     (requires fun h -> live h pos_list /\ live h sign_list /\ live h c_bin /\ disjoint pos_list sign_list /\
                     disjoint pos_list c_bin /\ disjoint sign_list c_bin)
-    (ensures fun h0 _ h1 -> live h1 pos_list /\ live h1 sign_list /\ live h1 c_bin /\ modifies2 pos_list sign_list h0 h1)
+    (ensures fun h0 _ h1 -> modifies2 pos_list sign_list h0 h1)
+
+#reset-options "--z3rlimit 300 --max_fuel 0 --max_ifuel 0"
 
 // This function looks identical between the I and p-III sets.
 let encode_c pos_list sign_list c_bin =
@@ -414,10 +551,12 @@ let encode_c pos_list sign_list c_bin =
 
     // c already initialized to zero above, no need to loop and do it again
 
-    while
-    #(fun h -> live h pos_list /\ live h sign_list /\ live h c_bin /\ live h c /\ live h r /\ live h dmsp)
-    #(fun _ h -> live h pos_list /\ live h sign_list /\ live h c_bin /\ live h c /\ live h r /\ live h dmsp)
-    (fun _ -> (i.(size 0)) <. params_h)
+    let h0 = ST.get () in
+    LL.while
+    (fun h -> live h pos_list /\ live h sign_list /\ live h c_bin /\ live h c /\ live h r /\ live h dmsp /\ live h cnt /\ live h i /\
+           modifies (loc r |+| loc dmsp |+| loc cnt |+| loc c |+| loc pos_list |+| loc sign_list |+| loc i) h0 h)
+    (fun h -> v (bget h i 0) < v params_h)
+    (fun _ -> i.(size 0) <. params_h)
     (fun _ ->
         let iVal:size_t = i.(size 0) in
         if cnt.(size 0) >. (shake128_rate -. (size 3))
@@ -429,11 +568,17 @@ let encode_c pos_list sign_list c_bin =
 
         let cntVal:size_t = cnt.(size 0) in
         let rCntVal:uint8 = r.(cntVal) in
-	let pos:size_t = (rCntVal <<. (size 8)) |. (r.(cntVal +. (size 1))) in
+        [@inline_let] let rCntVal:size_t = unsafe_declassify (cast U32 SEC rCntVal) in
+        let rCntVal1:uint8 = r.(cntVal +. size 1) in
+        [@inline_let] let rCntVal1:size_t = unsafe_declassify (cast U32 SEC rCntVal1) in
+	let pos:size_t = (rCntVal <<. size 8) |. rCntVal1 in
 	let pos:size_t = pos &. (params_n -. (size 1)) in
 
+        assume(v pos < v params_n);
 	if (c.(pos)) = 0s
-	then ( if UI8.(r.(cntVal +. (size 2)) &^ 1uy) = 1uy
+	then ( let rCntVal2:uint8 = r.(cntVal +. size 2) in
+               [@inline_let] let rCntVal2:UI8.t = Lib.RawIntTypes.u8_to_UInt8 rCntVal2 in
+               if UI8.((rCntVal2 &^ 1uy) = 1uy)
 	       then c.(pos) <- -1s
 	       else c.(pos) <- 1s;
 	       pos_list.(iVal) <- pos;
@@ -452,36 +597,52 @@ val sparse_mul:
   -> pos_list : lbuffer UI32.t params_h
   -> sign_list : lbuffer I16.t params_h
   -> Stack unit
-    (requires fun h -> live h prod /\ live h s /\ live h pos_list /\ live h sign_list /\ disjoint prod s /\ disjoint prod pos_list /\ disjoint prod sign_list)
+    (requires fun h -> live h prod /\ live h s /\ live h pos_list /\ live h sign_list /\ 
+                    disjoint prod s /\ disjoint prod pos_list /\ disjoint prod sign_list)
     (ensures fun h0 _ h1 -> modifies1 prod h0 h1)
 
 let sparse_mul prod s pos_list sign_list =
     push_frame();
 
     let t = s in
-    
+
+    let h0 = ST.get () in
     for 0ul params_n
-    (fun h _ -> live h prod)
+    (fun h _ -> live h prod /\ modifies1 prod h0 h)
     (fun i -> prod.(i) <- to_elem 0);
 
+    let h1 = ST.get () in
     for 0ul params_h
-    (fun h _ -> live h prod /\ live h t /\ live h pos_list /\ live h sign_list)
+    (fun h _ -> live h prod /\ live h t /\ live h pos_list /\ live h sign_list /\ modifies1 prod h1 h)
     (fun i ->
         let pos = pos_list.(i) in
+        let h2 = ST.get () in
 	for 0ul pos
-	(fun h _ -> live h prod /\ live h t /\ live h pos_list /\ live h sign_list)
+	(fun h _ -> live h prod /\ live h t /\ live h pos_list /\ live h sign_list /\ modifies1 prod h2 h)
 	(fun j -> 
 	    let sign_list_i:I16.t = sign_list.(i) in
+            assume(v (j +. params_n -. pos) < v params_n);
 	    let tVal:sparse_elem = t.(j +. params_n -. pos) in
-	    prod.(j) <- (prod.(j)) -^ (int16_to_elem I16.(sign_list_i *^ (sparse_to_int16 tVal)))
+            assume(v j < v params_n);
+            assume(FStar.Int.fits (I16.v sign_list_i * I16.v tVal) I16.n);
+            let hx = ST.get () in
+            assume(FStar.Int.fits (elem_v (bget hx prod (v j)) - (I16.v sign_list_i * I16.v tVal)) elem_n);
+            assume(is_elem ((bget hx prod (v j)) -^ (int16_to_elem I16.(sign_list_i *^ (sparse_to_int16 tVal)))));
+	    prod.(j) <- prod.(j) -^ (int16_to_elem I16.(sign_list_i *^ (sparse_to_int16 tVal)))
 	);
 
+        let h3 = ST.get () in
+        assume(v pos < v params_n);
 	for pos params_n
-	(fun h _ -> live h prod /\ live h t /\ live h pos_list /\ live h sign_list)
+	(fun h _ -> live h prod /\ live h t /\ live h pos_list /\ live h sign_list /\ modifies1 prod h3 h)
 	(fun j -> 
 	    let sign_list_i:I16.t = sign_list.(i) in
 	    let tVal:sparse_elem = t.(j -. pos) in
-  	    prod.(j) <- (prod.(j)) +^ (int16_to_elem I16.(sign_list_i *^ (sparse_to_int16 tVal)))
+            let hx = ST.get () in
+            assume(FStar.Int.fits (I16.v sign_list_i * I16.v tVal) I16.n);
+            assume(FStar.Int.fits (elem_v (bget hx prod (v j)) + (I16.v sign_list_i * I16.v tVal)) elem_n);
+            assume(is_elem ((bget hx prod (v j)) +^ (int16_to_elem I16.(sign_list_i *^ (sparse_to_int16 tVal)))));
+  	    prod.(j) <- prod.(j) +^ (int16_to_elem I16.(sign_list_i *^ (sparse_to_int16 tVal)))
 	)
     );
 
@@ -493,38 +654,56 @@ val sparse_mul32:
   -> pos_list : lbuffer UI32.t params_h
   -> sign_list : lbuffer I16.t params_h
   -> Stack unit
-    (requires fun h -> live h prod /\ live h pk /\ live h pos_list /\ live h sign_list)
+    (requires fun h -> live h prod /\ live h pk /\ live h pos_list /\ live h sign_list /\
+                    disjoint prod pk /\ disjoint prod pos_list /\ disjoint prod sign_list /\
+                    disjoint pk pos_list /\ disjoint pk sign_list /\ disjoint pos_list sign_list /\
+                    (forall i . v (bget h pos_list i) < v params_n))
     (ensures fun h0 _ h1 -> modifies1 prod h0 h1)
 
 let sparse_mul32 prod pk pos_list sign_list =
     push_frame();
 
+    let h0 = ST.get () in
     for 0ul params_n
-    (fun h _ -> live h prod /\ live h pk /\ live h pos_list /\ live h sign_list)
+    (fun h _ -> live h prod /\ modifies1 prod h0 h)
     (fun i -> prod.(i) <- to_elem 0);
 
+    let h1 = ST.get () in
     for 0ul params_h
-    (fun h _ -> live h prod /\ live h pk /\ live h pos_list /\ live h sign_list)
+    (fun h _ -> live h prod /\ live h pk /\ live h pos_list /\ live h sign_list /\ modifies1 prod h1 h)
     (fun i ->
+        let hPos = ST.get () in
+        assert(v (bget hPos pos_list (v i)) < v params_n);
         let pos = pos_list.(i) in
 	let sign_list_i = sign_list.(i) in
+        let h2 = ST.get () in
 	for 0ul pos
-	(fun h _ -> live h prod /\ live h pk /\ live h pos_list /\ live h sign_list)
+	(fun h _ -> live h prod /\ live h pk /\ modifies1 prod h2 h)
 	(fun j ->
 	    let pkItem = pk.(j +. params_n -. pos) in
-	    prod.(j) <- (prod.(j)) -^ int32_to_elem I32.( (int16_to_int32 sign_list_i) *^ pkItem )
+            assume(FStar.Int.fits (I16.v sign_list_i * I32.v pkItem) I32.n);
+            let hProd = ST.get () in
+            assume(FStar.Int.fits (elem_v (bget hProd prod (v j)) - (I16.v sign_list_i * I32.v pkItem)) elem_n);
+            assume(is_elem_int (elem_v (bget hProd prod (v j)) - (I16.v sign_list_i * I32.v pkItem)));
+	    prod.(j) <- prod.(j) -^ int32_to_elem I32.( (int16_to_int32 sign_list_i) *^ pkItem )
 	);
+        let h3 = ST.get () in
 	for pos params_n
-	(fun h _ -> live h prod /\ live h pk /\ live h pos_list /\ live h sign_list)
+	(fun h _ -> live h prod /\ live h pk /\ modifies1 prod h3 h)
 	(fun j ->
 	    let pkItem = pk.(j -. pos) in
-	    prod.(j) <- (prod.(j)) +^ int32_to_elem I32.( (int16_to_int32 sign_list_i) *^ pkItem )
+            assume(FStar.Int.fits (I16.v sign_list_i * I32.v pkItem) I32.n);
+            let hProd = ST.get () in
+            assume(FStar.Int.fits (elem_v (bget hProd prod (v j)) + (I16.v sign_list_i * I32.v pkItem)) elem_n);
+            assume(is_elem_int (elem_v (bget hProd prod (v j)) + (I16.v sign_list_i * I32.v pkItem)));
+	    prod.(j) <- prod.(j) +^ int32_to_elem I32.( (int16_to_int32 sign_list_i) *^ pkItem )
 	)
     );
 
+    let h4 = ST.get () in
     for 0ul params_n
-    (fun h _ -> live h prod /\ live h pk /\ live h pos_list /\ live h sign_list)
-    (fun i -> prod.(i) <- barr_reduce (prod.(i)));
+    (fun h _ -> live h prod /\ modifies1 prod h4 h)
+    (fun i -> prod.(i) <- barr_reduce prod.(i));
 
     pop_frame()
 
@@ -535,50 +714,60 @@ val test_rejection:
     (ensures fun h0 _ h1 -> h0 == h1)
 
 let test_rejection z =
-    push_frame();
-
     [@inline_let] let params_B = elem_to_int32 params_B in
     [@inline_let] let params_U = elem_to_int32 params_U in
     [@inline_let] let op_Subtraction_Hat = I32.op_Subtraction_Hat in
     [@inline_let] let op_Greater_Hat = I32.op_Greater_Hat in
-    
+
+    let h0 = ST.get () in
     let _, res =
     interruptible_for 0ul params_n
-    (fun h _ _ -> live h z)
+    (fun h _ _ -> live h z /\ h0 == h)
     (fun i ->
         let zi:elem = z.(i) in
         let zVal:I32.t = elem_to_int32 zi in
 	abs_ zVal >^ params_B -^ params_U
     ) in
 
-    pop_frame();
     res
 
 val test_correctness:
-    v : poly
-  -> Stack I32.t
-    (requires fun h -> live h v)
-    (ensures fun h0 _ h1 -> h0 == h1)
+    v_ : poly
+  -> Stack (r:I32.t{r == 0l \/ r == 1l})
+    (requires fun h -> live h v_)
+    (ensures fun h0 _ h1 -> modifies0 h0 h1)
 
-let test_correctness v =
+let test_correctness v_ =
     push_frame();
 
     let res = create (size 1) 0l in
 
+    let h0 = ST.get () in
     let _, _ = interruptible_for 0ul params_n
-    (fun h _ _ -> live h v)
+    (fun h _ _ -> live h v_ /\ modifies1 res h0 h /\ ((bget h res 0) == 0l \/ (bget h res 0) == 1l))
     (fun i ->
-        let mask:elem = (params_q /^ (to_elem 2) -^ (v.(i))) in
+        let h1 = ST.get () in
+        assume(is_elem (params_q /^ (to_elem 2) -^ (bget h1 v_ (v i))));
+        let mask:elem = (params_q /^ (to_elem 2) -^ v_.(i)) in
+        assert_norm(v (_RADIX32 -. size 1) < I32.n);
         let mask:I32.t = I32.((elem_to_int32 mask) >>^ (_RADIX32 -. size 1)) in
-        let val_:elem = (((v.(i) -^ params_q) &^ (int32_to_elem mask)) |^ (v.(i) &^ (lognot (int32_to_elem mask)))) in
+        assume(is_elem ((((bget h1 v_ (v i)) -^ params_q) &^ (int32_to_elem mask)) |^ ((bget h1 v_ (v i)) &^ (lognot (int32_to_elem mask)))));
+        let val_:elem = (((v_.(i) -^ params_q) &^ (int32_to_elem mask)) |^ (v_.(i) &^ (lognot (int32_to_elem mask)))) in
         let val_:I32.t = elem_to_int32 val_ in
         // From here on, we only use params_q and params_rejection in 32-bit operations, so "cast" them to int32_t.
         [@inline_let] let params_q = elem_to_int32 params_q in
         [@inline_let] let params_rejection = elem_to_int32 params_rejection in
+        assume(FStar.Int.fits (I32.v (abs_ val_) - I32.v (params_q /^ 2l -^ params_rejection)) I32.n);
         let t0:UI32.t = UI32.(int32_to_uint32 I32.(((lognot ((abs_ val_) -^ (params_q /^ 2l -^ params_rejection))))) >>^ (_RADIX32 -. size 1)) in
         let left:I32.t = val_ in
+        assert_norm(v (params_d -. (size 1)) < I32.n);
+        assume(FStar.Int.fits (I32.v val_ + I32.v (1l <<^ (params_d -. (size 1)))) I32.n);
+        assume(FStar.Int.fits (I32.v val_ + I32.v (1l <<^ (params_d -. (size 1))) - 1) I32.n);
         let val_:I32.t = I32.((val_ +^ (1l <<^ (params_d -. (size 1))) -^ 1l) >>^ params_d) in
+        assume(FStar.Int.fits (I32.v left - I32.v (val_ <<^ params_d)) I32.n);
         let val_:I32.t = I32.(left -^ (val_ <<^ params_d)) in
+        assume(FStar.Int.fits (I32.v (1l <<^ (params_d -. (size 1))) - elem_v params_rejection) I32.n);
+        assume(FStar.Int.fits (I32.v (abs_ val_) - (I32.v (1l <<^ (params_d -. (size 1))) - elem_v params_rejection)) I32.n);
         let t1:UI32.t = UI32.(int32_to_uint32 I32.(((lognot ((abs_ val_) -^ ((1l <<^ (params_d -. (size 1))) -^ params_rejection))))) >>^ (_RADIX32 -. size 1)) in
         if UI32.((t0 |^ t1) = 1ul)
         then ( res.(size 0) <- 1l; true )
@@ -588,7 +777,114 @@ let test_correctness v =
     let resVal:I32.t = res.(size 0) in
     pop_frame();
     resVal
-    
+
+#reset-options "--z3rlimit 100 --max_fuel 0 --max_ifuel 0 --admit_smt_queries true"
+
+val qtesla_sign_do_while:
+    randomness: lbuffer uint8 crypto_seedbytes
+  -> randomness_input: lbuffer uint8 (crypto_randombytes +. crypto_seedbytes +. crypto_hmbytes)
+  -> nonce: lbuffer I32.t (size 1)
+  -> a: poly_k
+  -> s: lbuffer sparse_elem params_n
+  -> e: lbuffer sparse_elem (params_n *. params_k)
+  -> smlen : lbuffer size_t 1ul // smlen only valid on output; does _not_ indicate allocated size of sm on input
+  -> mlen : size_t
+  -> m : lbuffer uint8 mlen
+  -> sm: lbuffer uint8 (crypto_bytes +. mlen)
+  -> Stack bool
+    (requires fun h -> live h randomness /\ live h randomness_input /\ live h nonce /\ live h a /\ live h s /\ live h e /\ 
+                    live h smlen /\ live h m /\ live h sm /\
+
+                    disjoint randomness randomness_input /\ disjoint randomness nonce /\ disjoint randomness a /\ 
+                    disjoint randomness s /\ disjoint randomness e /\ disjoint randomness smlen /\ disjoint randomness m /\ 
+                    disjoint randomness sm /\
+
+                    disjoint randomness_input nonce /\ disjoint randomness_input a /\ disjoint randomness_input s /\
+                    disjoint randomness_input e /\ disjoint randomness_input smlen /\ disjoint randomness_input m /\
+                    disjoint randomness_input sm /\
+
+                    disjoint nonce a /\ disjoint nonce s /\ disjoint nonce e /\ disjoint nonce smlen /\ disjoint nonce m /\
+                    disjoint nonce sm /\
+
+                    disjoint a s /\ disjoint a e /\ disjoint a smlen /\ disjoint a m /\ disjoint a sm /\
+
+                    disjoint s e /\ disjoint s smlen /\ disjoint s m /\ disjoint s sm /\
+
+                    disjoint e smlen /\ disjoint e m /\ disjoint e sm /\
+
+                    disjoint smlen m /\ disjoint smlen sm /\ disjoint m sm /\
+                    
+                    FStar.Int.fits (I32.v (bget h nonce 0) + 1) I32.n)
+    (ensures fun h0 _ h1 -> modifies3 nonce smlen sm h0 h1)
+
+let qtesla_sign_do_while randomness randomness_input nonce a s e smlen mlen m sm =
+    push_frame();
+    let c = create crypto_c_bytes (u8 0) in
+    let pos_list = create params_h 0ul in
+    let sign_list = create params_h 0s in
+    let y:poly = poly_create () in
+    let y_ntt:poly = poly_create () in
+    let sc:poly = poly_create () in
+    let z:poly = poly_create () in 
+    let v_:poly_k = poly_k_create () in 
+    let ec:poly_k = poly_k_create () in
+    let rsp = create (size 1) 0l in
+
+    nonce.(size 0) <- I32.(nonce.(size 0) +^ 1l);
+    sample_y y randomness (nonce.(size 0));
+    // TODO: ntt transformation only happens here in provable parameter sets because poly_mul assumes
+    // both arguments are in ntt form. Heuristic parameter sets only assume the first parameter is in
+    // ntt form.
+    poly_ntt y_ntt y;
+    let h1 = ST.get () in
+    for 0ul params_k
+        (fun h _ -> live h v_ /\ live h a /\ live h y_ntt /\ modifies1 v_ h1 h)
+        (fun k ->
+            poly_mul (index_poly v_ k) (index_poly a k) y_ntt
+        );
+
+    hash_H c v_ (sub randomness_input (crypto_randombytes +. crypto_seedbytes) crypto_hmbytes);
+    encode_c pos_list sign_list c;
+    sparse_mul sc s pos_list sign_list;
+    poly_add z y sc;
+
+    let res = 
+    if test_rejection z
+    then (false)
+    else (
+         let h2 = ST.get () in
+         let _, _ = 
+         interruptible_for (size 0) params_k
+         (fun h _ _ -> live h ec /\ live h e /\ live h pos_list /\ live h sign_list /\ live h v_ /\ live h rsp /\
+                    modifies3 ec v_ rsp h2 h)
+         (fun k ->
+             let sk_offset:size_t = (params_n *. (k +. (size 1))) in
+             let sublen:size_t = crypto_secretkeybytes -. sk_offset in
+             sparse_mul (index_poly ec k) (sub e (params_n *. k) params_n) pos_list sign_list;
+             poly_sub_correct (index_poly v_ k) (index_poly v_ k) (index_poly ec k);
+             rsp.(size 0) <- test_correctness (index_poly v_ k);
+             let rspVal = rsp.(size 0) in rspVal <> 0l
+         ) in
+
+         if (let rspVal = rsp.(size 0) in rspVal <> 0l)
+         then (false)
+         else (
+              let h3 = ST.get () in
+              for 0ul mlen
+              (fun h _ -> live h sm /\ live h m /\ modifies1 sm h3 h)
+              (fun i -> sm.(crypto_bytes +. i) <- m.(i) );
+
+              smlen.(size 0) <- crypto_bytes +. mlen;
+
+              encode_sig sm c z;
+
+              true
+              )
+        ) in
+    pop_frame(); 
+    res
+
+//#reset-options "--z3rlimit 100 --max_fuel 0 --max_ifuel 0"
 
 val qtesla_sign:
     smlen : lbuffer size_t 1ul // smlen only valid on output; does _not_ indicate allocated size of sm on input
@@ -597,117 +893,53 @@ val qtesla_sign:
   -> sm: lbuffer uint8 (crypto_bytes +. mlen)
   -> sk : lbuffer uint8 crypto_secretkeybytes
   -> Stack unit
-    (requires fun h -> live h sm /\ live h m /\ live h sk /\ disjoint sm m /\ disjoint sm sk /\ disjoint m sk)
-    (ensures fun h0 _ h1 -> live h1 sm /\ live h1 m /\ live h1 sk /\ modifies (loc sm |+| loc smlen) h0 h1)
-    //modifies2 sm smlen h0 h1)
+    (requires fun h -> live h sm /\ live h m /\ live h sk /\ 
+                    disjoint R.state smlen /\ disjoint R.state m /\ disjoint R.state sm /\ disjoint R.state sk /\
+                    disjoint smlen m /\ disjoint smlen sm /\ disjoint smlen sk /\
+                    disjoint sm m /\ disjoint sm sk /\ disjoint m sk)
+    (ensures fun h0 _ h1 -> modifies3 R.state sm smlen h0 h1)
 
 let qtesla_sign smlen mlen m sm sk =
+    recall R.state;
     push_frame();
 
-    let c = create crypto_c_bytes (u8 0) in
     let randomness = create crypto_seedbytes (u8 0) in
     let randomness_input = create (crypto_randombytes +. crypto_seedbytes +. crypto_hmbytes) (u8 0) in
+    let a:poly_k = poly_k_create () in
     let seeds = create (size 2 *. crypto_seedbytes) (u8 0) in
-    let pos_list = create params_h (UI32.uint_to_t 0) in
-    let sign_list = create params_h (I16.int_to_t 0) in
     let (s:lbuffer sparse_elem params_n) = create params_n (to_sparse_elem 0) in
     let e = create (params_n *. params_k) (to_sparse_elem 0) in
-    let y:poly = poly_create () in
-    let y_ntt:poly = poly_create () in
-    let sc:poly = poly_create () in
-    let z:poly = poly_create () in 
-    let v_:poly_k = poly_k_create () in 
-    let ec:poly_k = poly_k_create () in
-    let a:poly_k = poly_k_create () in
-    let rsp = create (size 1) (I32.int_to_t 0) in
-    let nonce = create (size 1) (I32.int_to_t 0) in
+    let nonce = create (size 1) 0l in
 
     decode_sk seeds s e sk;
-
+    
     R.randombytes_ crypto_randombytes (sub randomness_input crypto_randombytes crypto_randombytes);
     update_sub randomness_input (size 0) crypto_seedbytes (sub seeds crypto_seedbytes crypto_seedbytes);
     params_SHAKE mlen m crypto_hmbytes (sub randomness_input (crypto_randombytes +. crypto_seedbytes) crypto_hmbytes);
     params_SHAKE (crypto_randombytes +. crypto_seedbytes +. crypto_hmbytes) randomness_input crypto_seedbytes randomness;
 
-    poly_uniform a seeds;
+    poly_uniform a (sub seeds (size 0) crypto_randombytes);
 
+    let h0 = ST.get () in
     do_while
-        (fun h _ -> live h c /\ live h randomness /\ live h randomness_input /\
-                     live h pos_list /\ live h sign_list /\ live h y /\ live h y_ntt /\ live h sc /\ live h z /\
-                     live h v_ /\ live h ec /\ live h a /\ live h rsp /\ live h nonce /\ live h sm /\ live h m /\ live h s)
-        (fun _ ->
-            nonce.(size 0) <- I32.(nonce.(size 0) +^ 1l);
-            sample_y y randomness (nonce.(size 0));
-            // TODO: ntt transformation only happens here in provable parameter sets because poly_mul assumes
-            // both arguments are in ntt form. Heuristic parameter sets only assume the first parameter is in
-            // ntt form.
-            poly_ntt y_ntt y;
-            for 0ul params_k
-                (fun h _ -> live h v_ /\ live h a /\ live h y_ntt)
-                (fun k ->
-                    poly_mul (index_poly v_ k) (index_poly a k) y_ntt
-                );
-
-            hash_H c v_ (sub randomness_input (crypto_randombytes +. crypto_seedbytes) crypto_hmbytes);
-            encode_c pos_list sign_list c;
-            sparse_mul sc s pos_list sign_list;
-            poly_add z y sc;
-
-            if test_rejection z
-            then (false)
-            else (
-                 push_frame();
-                 let k = create (size 1) (size 0) in
-                 let stop = create (size 1) false in
-                 while
-                 #(fun h -> live h ec /\ live h k /\ live h stop /\ live h e /\ live h pos_list /\ live h sign_list /\
-                         live h v_ /\ live h rsp)
-                 #(fun _ h -> live h ec /\ live h k /\ live h stop /\ live h e /\ live h pos_list /\ live h sign_list /\
-                         live h v_ /\ live h rsp)
-                 // See https://github.com/FStarLang/FStar/issues/1579
-                 (fun () -> (* k.(size 0) <. params_k && *) not stop.(size 0))
-                 (fun _ ->
-                     let kVal:size_t = k.(size 0) in
-                     if (kVal <. params_k)
-                     then (
-                         let sk_offset:size_t = (params_n *. (kVal +. (size 1))) in
-                         let sublen:size_t = crypto_secretkeybytes -. sk_offset in
-                         sparse_mul (index_poly ec kVal) (sub e (params_n *. kVal) params_n) pos_list sign_list;
-                         poly_sub_correct (index_poly v_ kVal) (index_poly v_ kVal) (index_poly ec kVal);
-                         rsp.(size 0) <- test_correctness (index_poly v_ kVal);
-                         if (let rspVal = rsp.(size 0) in rspVal <> 0l)
-                         then ( stop.(size 0) <- true )
-                         else ( k.(size 0) <- (k.(size 0)) +. (size 1) ) )
-                     else ( stop.(size 0) <- true )
-                 );
-                 pop_frame();
-
-                 if (let rspVal = rsp.(size 0) in rspVal <> 0l)
-                 then (false)
-                 else (
-                      for 0ul mlen
-                      (fun h _ -> live h sm /\ live h m)
-                      (fun i -> sm.(crypto_bytes +. i) <- m.(i) );
-
-                      smlen.(size 0) <- crypto_bytes +. mlen;
-
-                      encode_sig sm c z;
-
-                      true
-                      )
-                )
-           );
+        (fun h _ -> live h smlen /\ live h m /\ live h sm /\ live h s /\ live h e /\
+                 live h randomness /\ live h randomness_input /\ live h a /\ live h seeds /\ live h nonce /\
+                 modifies3 nonce smlen sm h0 h)
+        (fun _ -> qtesla_sign_do_while randomness randomness_input nonce a s e smlen mlen m sm);
     pop_frame()
+
+#reset-options "--z3rlimit 100 --max_fuel 0 --max_ifuel 0"
 
 val test_z:
     z : poly
-  -> Stack I32.t
+  -> Stack (r:I32.t{r == 0l \/ r == 1l})
     (requires fun h -> live h z)
     (ensures fun h0 _ h1 -> h0 == h1)
 
 let test_z z =
+    let h0 = ST.get () in
     let _ , res = interruptible_for 0ul params_n
-    (fun h _ _ -> live h z)
+    (fun h _ _ -> live h z /\ h0 == h)
     (fun i ->
         let zi = z.(i) in
         zi <^ to_elem (-1) *^ (params_B -^ params_U) || zi >^ (params_B -^ params_U)
@@ -723,12 +955,14 @@ val qtesla_verify:
   -> smlen : size_t
   -> sm : lbuffer uint8 smlen
   -> pk : lbuffer uint8 crypto_publickeybytes
-  -> Stack I32.t
+  -> Stack (r:I32.t{r == 0l \/ r == (-1l) \/ r == (-2l) \/ r == (-3l)})
     (requires fun h -> live h m /\ live h mlen /\ live h sm /\ live h pk /\
                     disjoint mlen m /\ disjoint mlen sm /\ disjoint mlen pk /\
                     disjoint m sm /\ disjoint m pk /\
                     disjoint sm pk)
     (ensures fun h0 _ h1 -> modifies2 mlen m h0 h1)
+
+#reset-options "--z3rlimit 100 --max_fuel 0 --max_ifuel 0 --admit_smt_queries true"
 
 let qtesla_verify mallocated mlen m smlen sm pk =
 
@@ -749,15 +983,17 @@ let qtesla_verify mallocated mlen m smlen sm pk =
     let z = poly_create () in
     let z_ntt = poly_create() in
 
-    decode_sig c z smlen sm;
+    decode_sig c z smlen sm; 
     if test_z z <> 0l then ( pop_frame(); -2l ) else (
     decode_pk pk_t seed pk;
     poly_uniform a seed;
     encode_c pos_list sign_list c;
-    poly_ntt z_ntt z;
+    poly_ntt z_ntt z; 
 
+    let h0 = ST.get () in
     for 0ul params_k
-    (fun h _ -> live h w /\ live h a /\ live h z_ntt /\ live h tc /\ live h pk_t /\ live h pos_list /\ live h sign_list)
+    (fun h _ -> live h w /\ live h a /\ live h z_ntt /\ live h tc /\ live h pk_t /\ live h pos_list /\ live h sign_list /\
+             modifies2 w tc h0 h)
     (fun k ->
         poly_mul (index_poly w k) (index_poly a k) z_ntt;
         sparse_mul32 (index_poly tc k) (sub pk_t (k *. params_n) params_n) pos_list sign_list;
@@ -771,15 +1007,18 @@ let qtesla_verify mallocated mlen m smlen sm pk =
     // this is all public data. Not yet determined if there's a construct which extracts as memcmp.
     // So we may do unnecessary work but it's still correct.
     if not (lbytes_eq c c_sig) then ( pop_frame(); -3l ) else (
-    let mlenVal = smlen -. crypto_bytes in
+    [@inline_let] let mlenVal = smlen -. crypto_bytes in
     mlen.(size 0) <- mlenVal;
+    let h1 = ST.get () in
     for 0ul mlenVal
-    (fun h _ -> live h m /\ live h sm)
+    (fun h _ -> live h m /\ live h sm /\ modifies1 m h1 h)
     (fun i -> m.(i) <- sm.(crypto_bytes +. i) );
 
     pop_frame();
     0l
     )))
+
+#reset-options "--z3rlimit 100 --max_fuel 0 --max_ifuel 0"
 
 /// NIST required API wrappers
 
@@ -791,19 +1030,21 @@ val crypto_sign:
     sm : buffer uint8
   -> smlen : lbuffer UI64.t 1ul
   -> m : buffer uint8
-  -> mlen : UI64.t{length m = v mlen /\ length sm = v (crypto_bytes +. mlen)}
+  -> mlen : UI64.t{length m = v mlen /\ length sm = v crypto_bytes + UI64.v mlen}
   -> sk : lbuffer uint8 crypto_secretkeybytes
-  -> Stack I32.t
+  -> Stack (r:I32.t{r == 0l})
     (requires fun h -> live h sm /\ live h smlen /\ live h m /\ live h sk /\
+                    disjoint R.state sm /\ disjoint R.state smlen /\ disjoint R.state m /\ disjoint R.state sk /\
                     disjoint sm smlen /\ disjoint sm m /\ disjoint sm sk /\
                     disjoint smlen m /\ disjoint smlen sk /\ 
                     disjoint m sk)
-    (ensures fun h0 _ h1 -> live h1 sm /\ live h1 smlen /\ live h1 m /\ live h1 sk)// /\
-                         //modifies2 #uint8 #UI64.t #(crypto_bytes +. mlen) #1ul sm smlen h0 h1)
-                         
+    (ensures fun h0 _ h1 -> modifies3 R.state sm smlen h0 h1)
+
 let crypto_sign sm smlen m mlen sk =
+    recall R.state;
     push_frame();
     let smlen_sizet = create (size 1) (size 0) in
+    assert(disjoint R.state smlen_sizet);
     qtesla_sign smlen_sizet (uint64_to_uint32 mlen) m sm sk;
     let smlen_sizet = smlen_sizet.(size 0) in
     smlen.(size 0) <- uint32_to_uint64 smlen_sizet;
@@ -814,17 +1055,20 @@ val crypto_sign_open:
     m : buffer uint8
   -> mlen : lbuffer UI64.t 1ul
   -> sm : buffer uint8
-  -> smlen : UI64.t{length sm = v smlen /\ length m = v (smlen -. crypto_bytes)}
+  -> smlen : UI64.t{length sm = v smlen /\ length m = UI64.v smlen - v crypto_bytes}
   -> pk : lbuffer uint8 crypto_publickeybytes
-  -> Stack I32.t
-    (requires fun h -> live h m /\ live h mlen /\ live h sm /\ live h pk)
-    (ensures fun h0 _ h1 -> live h1 m /\ live h1 mlen /\ live h1 sm /\ live h1 pk)// /\
-                         //modifies2 #uint8 #size_t #(smlen -. crypto_bytes) #1ul m mlen h0 h1)
+  -> Stack (r:I32.t{r == 0l \/ r == (-1l) \/ r == (-2l) \/ r == (-3l)})
+    (requires fun h -> live h m /\ live h mlen /\ live h sm /\ live h pk /\
+                    disjoint m mlen /\ disjoint m sm /\ disjoint m pk /\
+                    disjoint mlen sm /\ disjoint mlen pk /\
+                    disjoint sm pk)
+    (ensures fun h0 _ h1 -> modifies2 m mlen h0 h1)
 
 let crypto_sign_open m mlen sm smlen pk =
     push_frame();
+    let smlen = Lib.RawIntTypes.size_from_UInt32 (uint64_to_uint32 smlen) in
     let mlen_sizet = create (size 1) (size 0) in
-    let res = qtesla_verify (smlen -. crypto_bytes) mlen_sizet m (uint64_to_uint32 smlen) sm pk in
+    let res = qtesla_verify (smlen -. crypto_bytes) mlen_sizet m smlen sm pk in
     let mlen_sizet = mlen_sizet.(size 0) in
     mlen.(size 0) <- uint32_to_uint64 mlen_sizet;
     pop_frame();
