qtesla/code/params-I/Hacl.Impl.QTesla.Pack.fst
@@ -2,6 +2,7 @@ module Hacl.Impl.QTesla.Pack
 
 open FStar.HyperStack
 open FStar.HyperStack.ST
+module ST = FStar.HyperStack.ST
 open FStar.Mul
 
 module SHA3 = Hacl.SHA3
@@ -22,11 +23,55 @@ open Lib.Buffer
 open Lib.ByteBuffer
 
 open C.Loops
+module LL = Lib.Loops
 
 open Hacl.Impl.QTesla.Params
 open Hacl.Impl.QTesla.Globals
 
-#reset-options "--z3rlimit 100 --max_fuel 0 --max_ifuel 0 --admit_smt_queries true"
+#reset-options "--z3rlimit 100 --max_fuel 1 --max_ifuel 1"
+
+private inline_for_extraction noextract
+val encode_sk_s:
+    sk: lbuffer uint8 crypto_secretkeybytes
+  -> s: poly
+  -> j: size_t
+  -> Stack size_t
+    (requires fun h -> live h sk /\ live h s /\ disjoint sk s)
+    (ensures fun h0 _ h1 -> modifies1 sk h0 h1)
+
+let encode_sk_s sk s j =
+    push_frame();
+    let iBuf = create (size 1) (size 0) in
+    let jBuf = create (size 1) j in
+
+    let h0 = ST.get () in
+    assert_norm(v crypto_secretkeybytes > 0); 
+    LL.while
+    (fun h -> live h iBuf /\ live h jBuf /\ live h sk /\ live h s /\ modifies3 sk iBuf jBuf h0 h)
+    (fun h -> v (bget h iBuf 0) < v params_n)
+    (fun _ -> iBuf.(size 0) <. params_n)
+    (fun _ ->
+        let i = iBuf.(size 0) in
+	let j = jBuf.(size 0) in
+
+        assume(v i + 3 < v params_n);
+        let si0 = s.(i+.size 0) in    let si1 = s.(i+.size 1) in
+	let si2 = s.(i+.size 2) in    let si3 = s.(i+.size 3) in
+	
+        assume(v j + 4 < v crypto_secretkeybytes);
+	sk.(j+.size 0) <- elem_to_uint8 si0;
+	sk.(j+.size 1) <- elem_to_uint8 (((si0 >>^ 8ul) &^ 0x03l) |^ (si1 <<^ 2ul));
+	sk.(j+.size 2) <- elem_to_uint8 (((si1 >>^ 6ul) &^ 0x0Fl) |^ (si2 <<^ 4ul));
+	sk.(j+.size 3) <- elem_to_uint8 (((si2 >>^ 4ul) &^ 0x3Fl) |^ (si3 <<^ 6ul));
+	sk.(j+.size 4) <- elem_to_uint8 (si3 >>^ 2ul);
+
+        jBuf.(size 0) <- j +. size 5;
+	iBuf.(size 0) <- i +. size 4
+    );
+
+    let j = jBuf.(size 0) in
+    pop_frame();
+    j
 
 val encode_sk:
     sk: lbuffer uint8 crypto_secretkeybytes
@@ -42,90 +87,51 @@ val encode_sk:
 let encode_sk sk s e seeds =
     push_frame();
 
-    let iBuf = create (size 1) (size 0) in
-    let jBuf = create (size 1) (size 0) in
-
-    while
-    #(fun h -> live h iBuf /\ live h jBuf /\ live h sk /\ live h s)
-    #(fun _ h -> live h iBuf /\ live h jBuf /\ live h sk /\ live h s)
-    (fun _ -> iBuf.(size 0) <. params_n)
-    (fun _ ->
-        let i = iBuf.(size 0) in
-	let j = jBuf.(size 0) in
-	
-        let si0 = s.(i+.size 0) in    let si1 = s.(i+.size 1) in
-	let si2 = s.(i+.size 2) in    let si3 = s.(i+.size 3) in
-	
-	sk.(j+.size 0) <- elem_to_uint8 si0;
-	sk.(j+.size 1) <- elem_to_uint8 (((si0 >>^ 8ul) &^ 0x03l) |^ (si1 <<^ 2ul));
-	sk.(j+.size 2) <- elem_to_uint8 (((si1 >>^ 6ul) &^ 0x0Fl) |^ (si2 <<^ 4ul));
-	sk.(j+.size 3) <- elem_to_uint8 (((si2 >>^ 4ul) &^ 0x3Fl) |^ (si3 <<^ 6ul));
-	sk.(j+.size 4) <- elem_to_uint8 (si3 >>^ 2ul);
-
-        jBuf.(size 0) <- j +. size 5;
-	iBuf.(size 0) <- i +. size 4
-    );
-
-    iBuf.(size 0) <- size 0;
+    let j = encode_sk_s sk s (size 0) in
+    let _ = encode_sk_s sk e j in
     
-    while
-    #(fun h -> live h iBuf /\ live h jBuf /\ live h sk /\ live h e)
-    #(fun _ h -> live h iBuf /\ live h jBuf /\ live h sk /\ live h e)
-    (fun _ -> iBuf.(size 0) <. params_n)
-    (fun _ ->
-        let i = iBuf.(size 0) in
-	let j = jBuf.(size 0) in
-
-        let ei0 = e.(i+.size 0) in    let ei1 = e.(i+.size 1) in
-	let ei2 = e.(i+.size 2) in    let ei3 = e.(i+.size 3) in
-	
-	sk.(j+.size 0) <- elem_to_uint8 ei0;
-	sk.(j+.size 1) <- elem_to_uint8 (((ei0 >>^ 8ul) &^ 0x03l) |^ (ei1 <<^ 2ul));
-	sk.(j+.size 2) <- elem_to_uint8 (((ei1 >>^ 6ul) &^ 0x0Fl) |^ (ei2 <<^ 4ul));
-	sk.(j+.size 3) <- elem_to_uint8 (((ei2 >>^ 4ul) &^ 0x3Fl) |^ (ei3 <<^ 6ul));
-	sk.(j+.size 4) <- elem_to_uint8 (ei3 >>^ 2ul);
-
-        jBuf.(size 0) <- j +. size 5;
-	iBuf.(size 0) <- i +. size 4
-    );
+    assume(v (size 2 *. params_s_bits *. params_n /. size 8) + v (size 2 *. crypto_seedbytes) < v crypto_secretkeybytes);
 
     update_sub #MUT #_ #_ sk (size 2 *. params_s_bits *. params_n /. size 8) (size 2 *. crypto_seedbytes) seeds;
 
     pop_frame()
-	
+
 inline_for_extraction noextract
 let encode_or_pack_sk = encode_sk
 
-val decode_sk:
-    seeds : lbuffer uint8 (size 2 *. crypto_seedbytes)
+private inline_for_extraction noextract
+val decode_sk_s:
+    j : size_t//{v j + 5 * v params_n <= v crypto_secretkeybytes}
   -> s : lbuffer I16.t params_n
-  -> e : lbuffer I16.t params_n
   -> sk : lbuffer uint8 crypto_secretkeybytes
-  -> Stack unit
-    (requires fun h -> live h seeds /\ live h s /\ live h e /\ live h sk /\
-                    disjoint seeds s /\ disjoint seeds e /\ disjoint seeds e /\
-		    disjoint s e /\ disjoint s sk /\ disjoint e sk)
-    // TODO: fix ensures clause		    
-    (ensures fun h0 _ h1 -> True) // modifies (loc_union (loc_union (loc_buffer seeds) (loc_buffer s)) (loc_buffer e)) h0 h1)
+  -> Stack size_t
+    (requires fun h -> live h s /\ live h sk /\ disjoint s sk)
+    (ensures fun h0 _ h1 -> modifies1 s h0 h1)
 
-let decode_sk seeds s e sk =
+let decode_sk_s j s sk =
     push_frame();
-
     let iBuf = create (size 1) (size 0) in
-    let jBuf = create (size 1) (size 0) in
+    let jBuf = create (size 1) j in
 
-    while
-    #(fun h -> live h s /\ live h sk /\ live h iBuf /\ live h jBuf)
-    #(fun _ h -> live h s /\ live h sk /\ live h iBuf /\ live h jBuf)
+    let h0 = ST.get () in
+    LL.while
+    (fun h -> live h s /\ live h sk /\ live h iBuf /\ live h jBuf /\ modifies3 s iBuf jBuf h0 h)// /\ 
+           //v (bget h jBuf 0) + 4 < v crypto_secretkeybytes) // Can't prove this yet. Assumed below.
+    (fun h -> v (bget h iBuf 0) < v params_n)
     (fun _ -> iBuf.(size 0) <. params_n)
     (fun _ ->
         let i = iBuf.(size 0) in
 	let j = jBuf.(size 0) in
 
-        let skj0 = sk.(j+.size 0) in    let skj1 = sk.(j+.size 1) in
-	let skj2 = sk.(j+.size 2) in    let skj3 = sk.(j+.size 3) in
-	let skj4 = sk.(j+.size 4) in
+        //assert_norm(v params_n / 5 < v crypto_secretkeybytes);
+        assume(v j + 4 < v crypto_secretkeybytes);
+        let skj0 = sk.(j+.size 0) in    [@inline_let] let skj0 = Lib.RawIntTypes.u8_to_UInt8 skj0 in    
+        let skj1 = sk.(j+.size 1) in    [@inline_let] let skj1 = Lib.RawIntTypes.u8_to_UInt8 skj1 in
+	let skj2 = sk.(j+.size 2) in    [@inline_let] let skj2 = Lib.RawIntTypes.u8_to_UInt8 skj2 in    
+        let skj3 = sk.(j+.size 3) in    [@inline_let] let skj3 = Lib.RawIntTypes.u8_to_UInt8 skj3 in
+	let skj4 = sk.(j+.size 4) in    [@inline_let] let skj4 = Lib.RawIntTypes.u8_to_UInt8 skj4 in
 
+        assume(v i + 3 < v params_n);
         s.(i+.size 0) <- I16.(uint8_to_int16 skj0               |^ int32_to_int16 I32.(((uint8_to_int32 skj1) <<^ 30ul) >>^ 22ul));
 	s.(i+.size 1) <- I16.(uint8_to_int16 UI8.(skj1 >>^ 2ul) |^ int32_to_int16 I32.(((uint8_to_int32 skj2) <<^ 28ul) >>^ 22ul));
 	s.(i+.size 2) <- I16.(uint8_to_int16 UI8.(skj2 >>^ 4ul) |^ int32_to_int16 I32.(((uint8_to_int32 skj3) <<^ 26ul) >>^ 22ul));
@@ -135,29 +141,35 @@ let decode_sk seeds s e sk =
 	iBuf.(size 0) <- i +. size 4
     );
 
-    iBuf.(size 0) <- size 0;
-    while
-    #(fun h -> live h e /\ live h sk /\ live h iBuf /\ live h jBuf)
-    #(fun _ h -> live h e /\ live h sk /\ live h iBuf /\ live h jBuf)
-    (fun _ -> iBuf.(size 0) <. params_n)
-    (fun _ ->
-        let i = iBuf.(size 0) in
-	let j = jBuf.(size 0) in
+    let j = jBuf.(size 0) in
+    pop_frame();
+    j
 
-        let skj0 = sk.(j+.size 0) in    let skj1 = sk.(j+.size 1) in
-	let skj2 = sk.(j+.size 2) in    let skj3 = sk.(j+.size 3) in
-	let skj4 = sk.(j+.size 4) in
+val decode_sk:
+    seeds : lbuffer uint8 (size 2 *. crypto_seedbytes)
+  -> s : lbuffer I16.t params_n
+  -> e : lbuffer I16.t params_n
+  -> sk : lbuffer uint8 crypto_secretkeybytes
+  -> Stack unit
+    (requires fun h -> live h seeds /\ live h s /\ live h e /\ live h sk /\
+                    disjoint seeds s /\ disjoint seeds e /\ disjoint seeds sk /\
+		    disjoint s e /\ disjoint s sk /\ disjoint e sk)
+    (ensures fun h0 _ h1 -> modifies3 seeds s e h0 h1)
 
-        e.(i+.size 0) <- I16.(uint8_to_int16 skj0               |^ int32_to_int16 I32.(((uint8_to_int32 skj1) <<^ 30ul) >>^ 22ul));
-	e.(i+.size 1) <- I16.(uint8_to_int16 UI8.(skj1 >>^ 2ul) |^ int32_to_int16 I32.(((uint8_to_int32 skj2) <<^ 28ul) >>^ 22ul));
-	e.(i+.size 2) <- I16.(uint8_to_int16 UI8.(skj2 >>^ 4ul) |^ int32_to_int16 I32.(((uint8_to_int32 skj3) <<^ 26ul) >>^ 22ul));
-	e.(i+.size 3) <- I16.(uint8_to_int16 UI8.(skj3 >>^ 6ul) |^ (int8_to_int16 (uint8_to_int8 skj4)) <<^ 2ul);
+let decode_sk seeds s e sk =
+    push_frame();
+    let h0 = ST.get () in
+    let j = decode_sk_s (size 0) s sk in
+    let h1 = ST.get () in
+    assert(modifies1 s h0 h1);
+    let _ = decode_sk_s j e sk in
+    let h2 = ST.get () in
+    assert(modifies2 s e h0 h2);
+    assume(v (size 2 *. params_s_bits *. params_n /. size 8) + v (size 2 *. crypto_seedbytes) < v crypto_secretkeybytes);
+    copy seeds (sub sk (size 2 *. params_s_bits *. params_n /. size 8) (size 2 *. crypto_seedbytes));  
 
-        jBuf.(size 0) <- j +. size 5;
-	iBuf.(size 0) <- i +. size 4
-    );
-
-    copy seeds (sub sk (size 2 *. params_s_bits *. params_n /. size 8) (size 2 *. crypto_seedbytes));
+    let h3 = ST.get () in
+    assert(modifies3 s e seeds h0 h3);
 
     pop_frame()
 
